Unified master-snapshot-style ghost state.
Committing prior to extending store_rel to interact with general
invariants (may be unsound).

mailbox/acq_rel_atomics.v
@@ -99,16 +99,18 @@ Context {state : Type}.
 
 (* Iris-weak gives a more in-depth encoding of protocol assertions in terms of invariants and ghost state. This
    simpler one is probably still sound and almost as powerful. *)
-Definition protocol_inv (ord : state -> state -> Prop) T l g g' := EX v : Z, EX s : state,
-  !!(repable_signed v) && data_at Tsh tint (vint v) l * ghost_master s g * ghost_var gsh1 s g' * T s v.
+Definition protocol_inv (ord : state -> state -> Prop) T l g := EX v : Z, EX s : state,
+  !!(repable_signed v) && data_at Tsh tint (vint v) l * ghost (gsh1, s) g * T s v.
 
-Definition protocol_R l g g' (s : state) ord T := invariant (protocol_inv ord T l g g') * ghost_snap s g.
+Definition protocol_piece (sh : share) l g (s : state) ord T :=
+  invariant (protocol_inv ord T l g) * ghost (sh, s) g.
 
-Definition protocol_W l g g' (s : state) ord T := invariant (protocol_inv ord T l g g') * ghost_var gsh2 s g'.
+Definition protocol_R := protocol_piece Share.bot.
+Definition protocol_W := protocol_piece gsh2.
 
-Lemma protocol_inv_super_non_expansive : forall n ord T l g g',
-  compcert_rmaps.RML.R.approx n (protocol_inv ord T l g g') =
-  compcert_rmaps.RML.R.approx n (protocol_inv ord (fun s v => compcert_rmaps.RML.R.approx n (T s v)) l g g').
+Lemma protocol_inv_super_non_expansive : forall n ord T l g,
+  compcert_rmaps.RML.R.approx n (protocol_inv ord T l g) =
+  compcert_rmaps.RML.R.approx n (protocol_inv ord (fun s v => compcert_rmaps.RML.R.approx n (T s v)) l g).
 Proof.
   intros; unfold protocol_inv.
   rewrite !approx_exp; apply f_equal; extensionality v.
@@ -116,21 +118,11 @@ Proof.
   rewrite !approx_sepcon, !approx_andp, approx_idem; auto.
 Qed.
 
-Lemma protocol_R_super_non_expansive : forall n l g g' s ord T,
-  compcert_rmaps.RML.R.approx n (protocol_R l g g' s ord T) =
-  compcert_rmaps.RML.R.approx n (protocol_R l g g' s ord (fun s v => compcert_rmaps.RML.R.approx n (T s v))).
+Lemma protocol_piece_super_non_expansive : forall n sh l g s ord T,
+  compcert_rmaps.RML.R.approx n (protocol_piece sh l g s ord T) =
+  compcert_rmaps.RML.R.approx n (protocol_piece sh l g s ord (fun s v => compcert_rmaps.RML.R.approx n (T s v))).
 Proof.
-  intros; unfold protocol_R.
-  rewrite !approx_sepcon; f_equal.
-  rewrite invariant_super_non_expansive; setoid_rewrite invariant_super_non_expansive at 2.
-  rewrite protocol_inv_super_non_expansive; auto.
-Qed.
-
-Lemma protocol_W_super_non_expansive : forall n l g g' s ord T,
-  compcert_rmaps.RML.R.approx n (protocol_W l g g' s ord T) =
-  compcert_rmaps.RML.R.approx n (protocol_W l g g' s ord (fun s v => compcert_rmaps.RML.R.approx n (T s v))).
-Proof.
-  intros; unfold protocol_W.
+  intros; unfold protocol_piece.
   rewrite !approx_sepcon; f_equal.
   rewrite invariant_super_non_expansive; setoid_rewrite invariant_super_non_expansive at 2.
   rewrite protocol_inv_super_non_expansive; auto.
@@ -138,104 +130,131 @@ Qed.
 
 Context `{PCM_order state}.
 
-Lemma protocol_R_duplicable : forall l g g' s T, duplicable (protocol_R l g g' s ord T).
+Lemma make_protocol_R : forall sh l g s T,
+  view_shift (protocol_piece sh l g s ord T) (protocol_piece sh l g s ord T * protocol_R l g s ord T).
 Proof.
-  intros; unfold protocol_R.
-  apply sepcon_duplicable; auto with dup.
-  apply ghost_snap_duplicable.
-Qed.
-
-Lemma protocol_W_R : forall l g g' s T,
-  view_shift (protocol_W l g g' s ord T) (protocol_W l g g' s ord T * protocol_R l g g' s ord T).
-Proof.
-  intros; unfold protocol_W, protocol_R.
+  intros; unfold protocol_W, protocol_R, protocol_piece.
   rewrite <- sepcon_assoc, (sepcon_comm _ (invariant _)), <- sepcon_assoc, <- general_atomics.invariant_duplicable.
   rewrite sepcon_assoc, !(sepcon_comm (invariant _)); apply invariant_view_shift.
   unfold protocol_inv.
-  rewrite !(later_exp' _ 0); view_shift_intro v.
-  rewrite !(later_exp' _ s); view_shift_intro s'.
-  rewrite !later_sepcon, !sepcon_assoc, !(sepcon_comm (|>(_ && _))).
-  rewrite sepcon_comm, !sepcon_assoc; etransitivity; [apply view_shift_sepcon1, ghost_timeless|].
-  etransitivity; [apply view_shift_sepcon1, master_snap|].
-  rewrite sepcon_comm, !sepcon_assoc; etransitivity; [apply view_shift_sepcon1, ghost_timeless|].
-  apply derives_view_shift.
-  assert_PROP (s' = s).
-  { rewrite <- !sepcon_assoc, (sepcon_comm _ (ghost_var gsh2 _ _)).
-    rewrite <- !sepcon_assoc, (sepcon_comm (ghost_var gsh2 _ _)).
-    setoid_rewrite ghost_var_share_join'; eauto; entailer!. }
-  Exists v; entailer!.
-  rewrite (later_exp' _ s); Exists s; rewrite !later_sepcon; entailer!.
-  apply now_later.
+  etransitivity; [apply view_shift_sepcon1, make_snap|].
+  rewrite (sepcon_comm _ (ghost _ _)); reflexivity.
 Qed.
 
-Lemma protocol_R_W : forall l g g' s s' T,
-  view_shift (protocol_W l g g' s ord T * protocol_R l g g' s' ord T) (!!(ord s' s) && protocol_W l g g' s ord T).
+Corollary protocol_R_duplicable : forall l g s T, duplicable (protocol_R l g s ord T).
 Proof.
-  intros; unfold protocol_W, protocol_R.
+  intros; apply make_protocol_R.
+Qed.
+
+Corollary protocol_W_R : forall l g s T,
+  view_shift (protocol_W l g s ord T) (protocol_W l g s ord T * protocol_R l g s ord T).
+Proof.
+  intros; apply make_protocol_R.
+Qed.
+
+Lemma protocol_R_W : forall l g s s' T,
+  view_shift (protocol_W l g s ord T * protocol_R l g s' ord T) (!!(ord s' s) && protocol_W l g s ord T).
+Proof.
+  intros; unfold protocol_W, protocol_R, protocol_piece.
   rewrite <- sepcon_assoc, (sepcon_comm _ (invariant _)), <- sepcon_assoc, <- general_atomics.invariant_duplicable.
   rewrite <- sepcon_andp_prop.
   rewrite sepcon_assoc, !(sepcon_comm (invariant _)); apply invariant_view_shift.
   unfold protocol_inv.
   rewrite !(later_exp' _ 0); view_shift_intro v.
   rewrite !(later_exp' _ s); view_shift_intro s0.
-  rewrite !later_sepcon, !sepcon_assoc, !(sepcon_comm (|>(_ && _))).
-  rewrite <- !sepcon_assoc, (sepcon_comm _ (|>ghost_master _ _)).
-  rewrite !sepcon_assoc; etransitivity; [apply view_shift_sepcon1, ghost_timeless|].
-  rewrite <- !sepcon_assoc, (sepcon_comm _ (ghost_snap _ _)), <- sepcon_assoc.
-  rewrite 3sepcon_assoc; etransitivity; [apply view_shift_sepcon1, master_snap_absorb_gen|].
-  rewrite <- !sepcon_assoc, (sepcon_comm _ (|>ghost_var _ _ _)).
-  rewrite !sepcon_assoc; etransitivity; [apply view_shift_sepcon1, ghost_timeless|].
-  apply derives_view_shift; Intros.
-  assert_PROP (s0 = s).
-  { rewrite <- !sepcon_assoc, (sepcon_comm _ (ghost_var gsh2 _ _)).
-    rewrite <- !sepcon_assoc, (sepcon_comm (ghost_var gsh2 _ _)).
-    setoid_rewrite ghost_var_share_join'; eauto; entailer!. }
-  Exists v; entailer!.
-  rewrite (later_exp' _ s); Exists s; rewrite !later_sepcon; entailer!.
-  apply now_later.
+  rewrite (sepcon_comm _ (ghost _ _)); setoid_rewrite snap_master_join.
+  apply derives_view_shift; Exists v; entailer!.
+  apply sepcon_derives; auto.
+  apply later_derives; Exists s0; entailer!.
+  { intro X; contradiction unreadable_bot; rewrite <- X; auto. }
 Qed.
 
-Lemma protocol_R_R : forall l g g' s1 s2 T, ord s1 s2 ->
-  protocol_R l g g' s1 ord T * protocol_R l g g' s2 ord T = protocol_R l g g' s2 ord T.
+Lemma protocol_R_join : forall l g s1 s2 s T, join s1 s2 s ->
+  protocol_R l g s1 ord T * protocol_R l g s2 ord T = protocol_R l g s ord T.
 Proof.
-  intros; unfold protocol_R.
+  intros; unfold protocol_R, protocol_piece.
   rewrite <- sepcon_assoc, (sepcon_comm _ (invariant _)), <- sepcon_assoc, <- general_atomics.invariant_duplicable.
-  erewrite sepcon_assoc, ghost_snap_join; eauto.
+  rewrite sepcon_assoc; setoid_rewrite ghost_snap_join; eauto; reflexivity.
+Qed.
+
+Corollary protocol_R_R : forall l g s1 s2 T, ord s1 s2 ->
+  protocol_R l g s1 ord T * protocol_R l g s2 ord T = protocol_R l g s2 ord T.
+Proof.
+  intros; apply protocol_R_join.
   apply join_comm, ord_join; auto.
 Qed.
 
-Lemma make_protocol : forall l v s T, repable_signed v ->
-  view_shift (data_at Tsh tint (vint v) l * T s v) (EX g : val, EX g' : val, protocol_W l g g' s ord T).
+Lemma protocol_R_join' : forall l g s1 s2 T,
+  protocol_R l g s1 ord T * protocol_R l g s2 ord T |--
+  EX s : _, !!(join s1 s2 s) && protocol_R l g s ord T.
 Proof.
   intros.
-  etransitivity; [apply ghost_alloc with (g := (Tsh, s)); auto with init|].
-  etransitivity; [apply ghost_alloc with (g := (@None state, Some s)), master_init|].
-  view_shift_intro g; view_shift_intro g'.
-  setoid_rewrite <- ghost_var_share_join; eauto.
-  etransitivity.
-  - rewrite <- !sepcon_assoc, (sepcon_comm _ (ghost_var gsh2 s g')), !sepcon_assoc.
-    apply view_shift_sepcon2.
-    apply make_inv with (Q := protocol_inv ord T l g g'); unfold protocol_inv.
-    Exists v s; entailer!.
-  - apply derives_view_shift; unfold protocol_W.
-    Exists g g'; cancel.
+  assert_PROP (joins s1 s2) as Hs;
+    [|destruct Hs as (s & ?); Exists s; entailer!; erewrite protocol_R_join; eauto].
+  unfold protocol_R, protocol_piece; rewrite <- sepcon_assoc, (sepcon_comm _ (invariant _)), <- sepcon_assoc,
+    <- general_atomics.invariant_duplicable, sepcon_assoc, sepcon_comm.
+  apply sepcon_derives_prop.
+  eapply derives_trans; [apply ghost_conflict|].
+  apply prop_left; intros ((s', ?) & ? & Hjoin); simpl in *; apply prop_right.
+  rewrite !eq_dec_refl in Hjoin; eexists; eauto.
 Qed.
 
-Lemma protocol_R_choose : forall l g g' s1 s2 T
-  (Hcompat : forall s2 s' s'', ord s1 s2 -> join s2 s' s'' -> exists s0, join s1 s' s0 /\ ord s0 s''),
-  view_shift (protocol_R l g g' s1 ord T * protocol_R l g g' s2 ord T) (protocol_R l g g' s1 ord T).
+Lemma make_protocol' : forall l g v s T, repable_signed v ->
+  view_shift (data_at Tsh tint (vint v) l * ghost_master s g * T s v) (protocol_W l g s ord T).
+Proof.
+  intros.
+  setoid_rewrite <- ghost_var_share_join; eauto.
+  unfold protocol_W.
+  rewrite !sepcon_assoc, (sepcon_comm (ghost_var gsh2 _ _)), <- !sepcon_assoc.
+  apply view_shift_sepcon1, make_inv.
+  unfold protocol_inv.
+  Exists v s; entailer!.
+Qed.
+
+Lemma make_protocol : forall l v s T, repable_signed v ->
+  view_shift (data_at Tsh tint (vint v) l * T s v) (EX g : val, protocol_W l g s ord T).
+Proof.
+  intros.
+  etransitivity; [apply ghost_alloc with (g := (Tsh, s)), master_init|].
+  view_shift_intro g; etransitivity; [etransitivity; [|apply make_protocol'; eauto]|].
+  - apply derives_view_shift; cancel.
+  - apply derives_view_shift; Exists g; auto.
+Qed.
+
+Lemma protocol_R_forget : forall l g s1 s2 T
+  (Hcompat : forall s' s'', ord s1 s2 -> join s2 s' s'' -> exists s0, join s1 s' s0 /\ ord s0 s''),
+  ord s1 s2 -> view_shift (protocol_R l g s2 ord T) (protocol_R l g s1 ord T).
 Proof.
   intros; unfold protocol_R.
+  apply view_shift_sepcon2, ghost_snap_forget; auto.
+Qed.
+
+Lemma protocol_R_choose : forall l g s1 s2 T
+  (Hcompat : forall s2 s' s'', ord s1 s2 -> join s2 s' s'' -> exists s0, join s1 s' s0 /\ ord s0 s''),
+  view_shift (protocol_R l g s1 ord T * protocol_R l g s2 ord T) (protocol_R l g s1 ord T).
+Proof.
+  intros; unfold protocol_R, protocol_piece.
   rewrite <- sepcon_assoc, (sepcon_comm _ (invariant _)), <- sepcon_assoc, <- general_atomics.invariant_duplicable.
   rewrite sepcon_assoc; apply view_shift_sepcon2, ghost_snap_choose; auto.
+Qed.
+
+Lemma protocol_piece_share_join : forall sh1 sh2 sh l g s1 s2 T (Hsh : sepalg.join sh1 sh2 sh)
+  (Hsh1 : readable_share sh1) (Hsh2 : readable_share sh2),
+  protocol_piece sh1 l g s1 ord T * protocol_piece sh2 l g s2 ord T =
+  !!(s1 = s2) && protocol_piece sh l g s1 ord T.
+Proof.
+  intros; unfold protocol_piece.
+  rewrite <- sepcon_assoc, (sepcon_comm _ (invariant _)), <- sepcon_assoc, <- general_atomics.invariant_duplicable.
+  rewrite sepcon_assoc; setoid_rewrite ghost_var_share_join'; eauto.
+  apply mpred_ext; entailer!.
 Qed.
 
 End protocols.
 
 Existing Instance max_PCM.
 
-Lemma protocol_R_choose' : forall l g g' s1 s2 T,
-  view_shift (protocol_R l g g' s1 Z.le T * protocol_R l g g' s2 Z.le T) (protocol_R l g g' s1 Z.le T).
+Lemma protocol_R_choose' : forall l g s1 s2 T,
+  view_shift (protocol_R l g s1 Z.le T * protocol_R l g s2 Z.le T) (protocol_R l g s1 Z.le T).
 Proof.
   intros; apply protocol_R_choose; simpl; intros; subst.
   do 2 eexists; eauto; apply Z.max_le_compat_r; auto.
@@ -244,26 +263,26 @@ Qed.
 Definition OrdType s := ArrowType s (ArrowType s (ConstType Prop)).
 Definition PredType s := ArrowType s (ArrowType (ConstType Z) Mpred).
 
-Definition LA_type := ProdType (ProdType (ProdType (ProdType (ProdType (ConstType (val * val * val))
+Definition LA_type := ProdType (ProdType (ProdType (ProdType (ProdType (ConstType (val * val))
   (DependentType 0)) (OrdType (DependentType 0))) (PredType (DependentType 0))) Mpred)
   (PredType (DependentType 0)).
 
 Program Definition load_acq_spec := TYPE LA_type
-  WITH l : val, g : val, g' : val, s : _, ord : _ -> _ -> Prop, T : _ -> Z -> mpred, P : mpred, Q : _ -> Z -> mpred
+  WITH l : val, g : val, s : _, ord : _ -> _ -> Prop, T : _ -> Z -> mpred, P : mpred, Q : _ -> Z -> mpred
   PRE [ 1%positive OF tptr tint ]
    PROP (forall s' v, ord s s' -> repable_signed v -> view_shift (P * T s' v) (P * T s' v * Q s' v)%logic;
          forall s' v, duplicable (Q s' v))
    LOCAL (temp 1%positive l)
-   SEP (protocol_R l g g' s ord T; P)
+   SEP (protocol_R l g s ord T; P)
   POST [ tint ]
    EX v : Z, EX s' : _,
    PROP (repable_signed v; ord s s')
    LOCAL (temp ret_temp (vint v))
-   SEP (protocol_R l g g' s' ord T; P; Q s' v).
+   SEP (protocol_R l g s' ord T; P; Q s' v).
 Next Obligation.
 Proof.
   repeat intro.
-  destruct x as (((((((?, ?), ?), s), ?), ?), ?), ?); simpl.
+  destruct x as ((((((?, ?), s), ?), ?), ?), ?); simpl.
   unfold PROPx; simpl; rewrite !approx_andp; f_equal.
   - rewrite !prop_and, !approx_andp; f_equal.
     + rewrite !prop_forall, !(approx_allp _ _ _ s); f_equal; extensionality s'.
@@ -276,93 +295,99 @@ Proof.
       rewrite !prop_forall, !(approx_allp _ _ _ 0); f_equal; extensionality v'.
       apply duplicable_super_non_expansive.
   - unfold LOCALx; simpl; rewrite !approx_andp; apply f_equal.
-    unfold SEPx; simpl; rewrite !approx_sepcon, protocol_R_super_non_expansive, approx_idem; auto.
+    unfold SEPx, protocol_R; simpl; rewrite !approx_sepcon, protocol_piece_super_non_expansive, approx_idem; auto.
 Qed.
 Next Obligation.
 Proof.
   repeat intro.
-  destruct x as (((((((?, ?), ?), ?), ?), ?), ?), ?); simpl.
+  destruct x as ((((((?, ?), ?), ?), ?), ?), ?); simpl.
   rewrite !approx_exp; apply f_equal; extensionality vr.
   rewrite !approx_exp; apply f_equal; extensionality s'.
   unfold PROPx; simpl; rewrite !approx_andp; apply f_equal.
   unfold LOCALx; simpl; rewrite !approx_andp; apply f_equal.
-  unfold SEPx; simpl; rewrite !approx_sepcon, protocol_R_super_non_expansive, !approx_idem; auto.
+  unfold SEPx, protocol_R; simpl; rewrite !approx_sepcon, protocol_piece_super_non_expansive, !approx_idem; auto.
 Qed.
 
-Definition SR_type := ProdType (ProdType (ProdType (ProdType (ProdType (ProdType (ConstType (val * Z * val * val))
+Definition SR_type := ProdType (ProdType (ProdType (ProdType (ProdType (ProdType (ConstType (val * Z * val))
   (DependentType 0)) (DependentType 0)) (OrdType (DependentType 0))) (PredType (DependentType 0))) Mpred) Mpred.
 
 (* single_writer version - multi-writer version uses protocol_R and requires that for all s',
    ord s s' -> ord s' s''. *)
+(* Using the stronger version from iGPS that allows the writer to pass its own protocol_W assertion into the
+   protocol invariant. *)
+(* Hypothesis: in the single-writer case, it's sound to allow the writer to interact with invariants. *)
 Program Definition store_rel_spec := TYPE SR_type
-  WITH l : val, v : Z, g : val, g' : val, s : _, s'' : _, st_ord : _ -> _ -> Prop, T : _ -> Z -> mpred, P : mpred, Q : mpred
+  WITH l : val, v : Z, g : val, s : _, s'' : _, st_ord : _ -> _ -> Prop, T : _ -> Z -> mpred, P : mpred, Q : mpred
   PRE [ 1%positive OF tptr tint, 2%positive OF tint ]
-   PROP (repable_signed v; forall v0, repable_signed v0 -> view_shift (P * T s v0) (T s'' v * Q); st_ord s s'')
+   PROP (repable_signed v; forall v0, repable_signed v0 ->
+     view_shift (P * protocol_W l g s st_ord T * T s v0)%logic (T s'' v * Q); st_ord s s'')
    LOCAL (temp 1%positive l; temp 2%positive (vint v))
-   SEP (protocol_W l g g' s st_ord T; P)
+   SEP (protocol_W l g s st_ord T; P)
   POST [ tvoid ]
    PROP ()
    LOCAL ()
-   SEP (protocol_W l g g' s'' st_ord T; Q).
+   SEP (protocol_R l g s'' st_ord T; Q).
 Next Obligation.
 Proof.
   repeat intro.
-  destruct x as (((((((((?, ?), ?), ?), ?), ?), ?), ?), ?), ?); simpl.
+  destruct x as ((((((((?, ?), ?), ?), ?), ?), ?), ?), ?); simpl.
   unfold PROPx; simpl; rewrite !approx_andp; f_equal.
   - rewrite !prop_and, !approx_andp; f_equal; f_equal.
     rewrite !prop_forall, !(approx_allp _ _ _ 0); f_equal; extensionality v'.
     rewrite !prop_impl; setoid_rewrite approx_imp; do 2 apply f_equal.
-    rewrite view_shift_super_non_expansive, !approx_sepcon; auto.
+    rewrite view_shift_super_non_expansive.
+    setoid_rewrite view_shift_super_non_expansive at 2.
+    unfold protocol_W; rewrite !approx_sepcon, protocol_piece_super_non_expansive, !approx_idem; auto.
   - unfold LOCALx; simpl; rewrite !approx_andp; apply f_equal.
-    unfold SEPx; simpl; rewrite !approx_sepcon, protocol_W_super_non_expansive, approx_idem; auto.
+    unfold SEPx, protocol_W; simpl; rewrite !approx_sepcon, protocol_piece_super_non_expansive, approx_idem; auto.
 Qed.
 Next Obligation.
 Proof.
   repeat intro.
-  destruct x as (((((((((?, ?), ?), ?), ?), ?), ?), ?), ?), ?); simpl.
+  destruct x as ((((((((?, ?), ?), ?), ?), ?), ?), ?), ?); simpl.
   unfold PROPx; simpl; rewrite !approx_andp; apply f_equal.
   unfold LOCALx; simpl; rewrite !approx_andp; apply f_equal.
-  unfold SEPx; simpl; rewrite !approx_sepcon, protocol_W_super_non_expansive, approx_idem; auto.
+  unfold SEPx, protocol_R; simpl; rewrite !approx_sepcon, protocol_piece_super_non_expansive, approx_idem; auto.
 Qed.
 
-Definition CRA_type := ProdType (ProdType (ProdType (ProdType (ProdType (ProdType (ConstType (val * Z * Z * val * val))
+Definition CRA_type := ProdType (ProdType (ProdType (ProdType (ProdType (ProdType (ConstType (val * Z * Z * val))
   (DependentType 0)) (DependentType 0)) (OrdType (DependentType 0))) (PredType (DependentType 0))) Mpred)
   (ArrowType (ConstType Z) Mpred).
 
 Program Definition CAS_RA_spec := TYPE CRA_type
-  WITH l : val, c : Z, v : Z, g : val, g' : val, s : _, s'' : _, ord : _ -> _ -> Prop, T : _ -> Z -> mpred,
+  WITH l : val, c : Z, v : Z, g : val, s : _, s'' : _, ord : _ -> _ -> Prop, T : _ -> Z -> mpred,
        P : mpred, Q : Z -> mpred
   PRE [ 1%positive OF tptr tint, 2%positive OF tint, 3%positive OF tint ]
    PROP (repable_signed c; repable_signed v; forall v0, repable_signed v0 ->
      view_shift (P * T s v0) ((if eq_dec v0 c then T s'' v else T s v0) * Q v0); ord s s'')
    LOCAL (temp 1%positive l; temp 2%positive (vint c); temp 3%positive (vint v))
-   SEP (protocol_W l g g' s ord T; P)
+   SEP (protocol_W l g s ord T; P)
   POST [ tint ]
    EX v' : Z,
    PROP (repable_signed v')
    LOCAL (temp ret_temp (Val.of_bool (if eq_dec v' c then true else false)))
-   SEP (protocol_W l g g' (if eq_dec v' c then s'' else s) ord T; Q v').
+   SEP (protocol_W l g (if eq_dec v' c then s'' else s) ord T; Q v').
 Next Obligation.
 Proof.
   repeat intro.
-  destruct x as ((((((((((?, ?), ?), ?), ?), ?), ?), ?), ?), ?), ?); simpl.
+  destruct x as (((((((((?, ?), ?), ?), ?), ?), ?), ?), ?), ?); simpl.
   unfold PROPx; simpl; rewrite !approx_andp; f_equal.
   - rewrite !prop_and, !approx_andp; do 2 apply f_equal; f_equal.
     rewrite !prop_forall, !(approx_allp _ _ _ 0); f_equal; extensionality v'.
     rewrite !prop_impl; setoid_rewrite approx_imp; do 2 apply f_equal.
     rewrite view_shift_super_non_expansive, !approx_sepcon; if_tac; auto.
   - unfold LOCALx; simpl; rewrite !approx_andp; f_equal.
-    unfold SEPx; simpl.
-    rewrite !approx_sepcon, protocol_W_super_non_expansive, approx_idem; auto.
+    unfold SEPx, protocol_W; simpl.
+    rewrite !approx_sepcon, protocol_piece_super_non_expansive, approx_idem; auto.
 Qed.
 Next Obligation.
 Proof.
   repeat intro.
-  destruct x as ((((((((((?, ?), ?), ?), ?), ?), ?), ?), ?), ?), ?); simpl.
+  destruct x as (((((((((?, ?), ?), ?), ?), ?), ?), ?), ?), ?); simpl.
   rewrite !approx_exp; apply f_equal; extensionality vr.
   unfold PROPx; simpl; rewrite !approx_andp; f_equal.
   unfold LOCALx; simpl; rewrite !approx_andp; f_equal.
-  unfold SEPx; simpl; rewrite !approx_sepcon, protocol_W_super_non_expansive, approx_idem; auto.
+  unfold SEPx, protocol_W; simpl; rewrite !approx_sepcon, protocol_piece_super_non_expansive, approx_idem; auto.
 Qed.
 
 End atomics.
