mailbox/verif_kvnode_atomic_ra.v
@@ -3,6 +3,7 @@ Require Import progs.ghost.
 Require Import mailbox.general_atomics.
 Require Import mailbox.acq_rel_atomics.
 Require Import progs.conclib.
+Require Import mailbox.maps.
 Require Import floyd.library.
 Require Import floyd.sublist.
 Require Import mailbox.kvnode_atomic_ra.
@@ -14,6 +15,18 @@ Definition Vprog : varspecs. mk_varspecs prog. Defined.
 
 Definition load_acq_spec := DECLARE _load_acq load_acq_spec.
 Definition store_rel_spec := DECLARE _store_rel store_rel_spec.
+
+Definition surely_malloc_spec :=
+ DECLARE _surely_malloc
+   WITH n:Z
+   PRE [ _n OF tuint ]
+       PROP (0 <= n <= Int.max_unsigned)
+       LOCAL (temp _n (Vint (Int.repr n)))
+       SEP ()
+    POST [ tptr tvoid ] EX p:_,
+       PROP ()
+       LOCAL (temp ret_temp p)
+       SEP (malloc_token Tsh n p * memory_block Tsh n p).
 
 Definition tnode := Tstruct _node noattr.
 
@@ -28,82 +41,114 @@ Proof.
   apply (proj2_sig has_size).
 Qed.
 
-(* Store a map from known version numbers to values. *)
-Instance version_PCM : PCM (Z -> option Z) := { join a b c :=
-  forall v1 v2, c v1 = Some v2 <-> a v1 = Some v2 \/ b v1 = Some v2 }.
-Proof.
-  - intros.
-    rewrite Hjoin; tauto.
-  - intros.
-    exists (fun v => match b v with Some v' => Some v' | None => d v end).
-    assert (forall v v1 v2, b v = Some v1 -> d v = Some v2 -> v1 = v2) as Hbd.
-    { intros ??? Hb Hd.
-      specialize (Hjoin1 v v1).
-      destruct Hjoin1 as (_ & Hc); lapply Hc; auto; intro Hc'.
-      generalize (Hjoin2 v v1); intros (_ & He); lapply He; auto; intro He1.
-      specialize (Hjoin2 v v2); destruct Hjoin2 as (_ & Hjoin2); lapply Hjoin2; auto; intro He2.
-      rewrite He1 in He2; inv He2; auto. }
-    split; intros; specialize (Hjoin1 v1 v2); specialize (Hjoin2 v1 v2).
-    + destruct (b v1) eqn: Hb; split; auto; intros [|]; auto; try discriminate.
-      exploit Hbd; eauto.
-    + rewrite Hjoin2, Hjoin1.
-      destruct (b v1) eqn: Hb; split; auto; intros [|]; auto.
-      * specialize (Hbd _ _ _ Hb H); subst; auto.
-      * destruct H; auto; discriminate.
-Defined.
-
-Definition log_incl (a b : Z -> option Z) := forall v1 v2, a v1 = Some v2 -> b v1 = Some v2.
-
-Instance version_order : PCM_order log_incl.
-Proof.
-  constructor.
-  - repeat intro; auto.
-  - repeat intro; auto.
-  - split; repeat intro; specialize (H v1 v2); rewrite H; auto.
-  - split; auto; intros [|]; auto.
-Defined.
-
-Definition log_latest s (v1 v2 : Z) := s v1 = Some v2 /\ forall v', v1 < v' -> s v' = None.
-
+(* Lexicographic ordering doesn't lead to a PCM (it's not associative), so we keep a full log of values. *)
 Definition data_T g s (v : Z) := EX ver : Z, !!(Z.even ver = true /\ log_latest s ver v) &&
   ghost_snap (ver - 1) g.
 
-Definition node_entry v vs locs g lg lg' i := EX log : _, !!(log_latest log v (Znth i vs 0)) &&
-  protocol_R (Znth i locs Vundef) (Znth i lg Vundef) (Znth i lg' Vundef) log log_incl (data_T g).
+Definition node_entry sh log locs g lg i :=
+  protocol_piece sh (Znth i locs Vundef) (Znth i lg Vundef) log map_incl (data_T g).
 
-Definition version_T locs g lg lg' (s v : Z) := !!(v = s) && EX vs : list Z,
-  fold_right sepcon emp (map (node_entry (if Z.even v then v else v - 1) vs locs g lg lg') (upto (Z.to_nat size))).
+Definition version_T locs g lg (s v : Z) := !!(v = s) && EX L : _,
+  !!(exists vs, log_latest L (if Z.even v then v else v - 1) vs) &&
+  fold_right sepcon emp (map (fun i => node_entry Share.bot (map_Znth i L 0) locs g lg i) (upto (Z.to_nat size))).
 
-Definition node_state v vs version locs g g' lg lg' := !!(Z.even v = true) &&
-  protocol_R version g g' v Z.le (version_T locs g lg lg') *
-  fold_right sepcon emp (map (node_entry v vs locs g lg lg') (upto (Z.to_nat size))).
+Definition node_state (sh : share) (L : Z -> option (list Z)) version locs g lg g' := EX v : Z, EX vs : list Z,
+  !!(Z.even v = true /\ log_latest L v vs) && protocol_piece sh version g v Z.le (version_T locs g lg) *
+  fold_right sepcon emp (map (fun i => node_entry sh (map_Znth i L 0) locs g lg i) (upto (Z.to_nat size))) *
+  ghost (sh, L) g'.
+
+Definition Ish := fst (Share.split gsh2).
+Definition Wsh := snd (Share.split gsh2).
+
+Lemma readable_Ish : readable_share Ish.
+Proof.
+  apply slice.split_YES_ok1; auto.
+Qed.
+
+Lemma readable_Wsh : readable_share Wsh.
+Proof.
+  apply slice.split_YES_ok2; auto.
+Qed.
+
+Lemma Ish_Wsh_join : sepalg.join Ish Wsh gsh2.
+Proof.
+  apply split_join; unfold Ish, Wsh; destruct (Share.split gsh2); auto.
+Qed.
+
+Hint Resolve readable_Ish readable_Wsh Ish_Wsh_join.
+
+(* It's useful to have both private and shared node_states, so we can know that whatever we read is at least
+   later than what we already knew. *)
+Program Definition read_spec := DECLARE _read atomic_spec
+  (ConstType (val * val * share * share * val * list val * val * val * list val *
+              (Z -> option (list Z)) * Z * list Z))
+  empty_map [(_n, tptr tnode); (_out, tptr tint)] tvoid
+  [fun _ '(n, out, sh, shi, version, locs, g, g', lg, L0, v0, vs0) => temp _n n;
+   fun _ '(n, out, sh, shi, version, locs, g, g', lg, L0, v0, vs0) => temp _out out]
+  (fun _ '(n, out, sh, shi, version, locs, g, g', lg, L0, v0, vs0) => !!(readable_share sh /\
+     writable_share shi /\ isptr version /\ Forall isptr locs /\ Zlength locs = size /\ log_latest L0 v0 vs0) &&
+   data_at sh tnode (version, locs) n * data_at_ shi (tarray tint size) out *
+   node_state Share.bot L0 version locs g lg g')
+  (fun _ '(n, out, sh, shi, version, locs, g, g', lg, L0, v0, vs0) L => node_state Ish L version locs g lg g')
+  (0, []) []
+  (fun _ '(n, out, sh, shi, version, locs, g, g', lg, L0, v0, vs0) L '(v, vals) =>
+   data_at sh tnode (version, locs) n * data_at shi (tarray tint size) (map (fun x => vint x) vals) out *
+   node_state Share.bot L version locs g lg g')
+  (fun _ '(n, out, sh, shi, version, locs, g, g', lg, L0, v0, vs0) L '(v, vals) =>
+   !!(map_incl L0 L /\ v0 <= v /\ L v = Some vals) && node_state Ish L version locs g lg g')
+  _ _ _ _ _ _.
+Next Obligation.
+Proof.
+  intros ?? w; decompose [prod] w; auto.
+Qed.
+Next Obligation.
+Proof.
+  intros ?? w; decompose [prod] w; auto.
+Qed.
+Next Obligation.
+Proof.
+  intros ?? w; decompose [prod] w; auto.
+Qed.
+Next Obligation.
+Proof.
+  intros ?? w; decompose [prod] w; auto.
+Qed.
+Next Obligation.
+Proof.
+  intros ?? w; decompose [prod] w; auto.
+Qed.
+Next Obligation.
+Proof.
+  intros ?? w; decompose [prod] w; auto.
+Qed.
+
+Definition node_entry_W L locs g lg i :=
+  protocol_W (Znth i locs Vundef) (Znth i lg Vundef) (map_Znth i L 0) map_incl (data_T g).
+
+Definition node_state_W L version locs g lg := EX v : Z, EX vs : list Z,
+  !!(Z.even v = true /\ log_latest L v vs) && protocol_W version g v Z.le (version_T locs g lg) *
+  fold_right sepcon emp (map (node_entry_W L locs g lg) (upto (Z.to_nat size))).
 
 Program Definition write_spec := DECLARE _write atomic_spec
-  (ConstType (val * val * share * share * val * list val * list Z * val * val * list val * list val * Z * list Z))
-  (0, []) [(_n, tptr tnode); (_in, tptr tint)] tvoid
-  [fun _ '(n, input, sh, shi, version, locs, vals, g, g', lg, lg', v0, vs0) => temp _n n;
-   fun _ '(n, input, sh, shi, version, locs, vals, g, g', lg, lg', v0, vs0) => temp _in input]
-  (fun _ '(n, input, sh, shi, version, locs, vals, g, g', lg, lg', v0, vs0) => !!(readable_share sh /\
+  (ConstType (val * val * share * share * val * list val * list Z * val * val * list val *
+              (Z -> option (list Z)) * Z * list Z))
+  empty_map [(_n, tptr tnode); (_in, tptr tint)] tvoid
+  [fun _ '(n, input, sh, shi, version, locs, vals, g, g', lg, L, v0, vs0) => temp _n n;
+   fun _ '(n, input, sh, shi, version, locs, vals, g, g', lg, L, v0, vs0) => temp _in input]
+  (fun _ '(n, input, sh, shi, version, locs, vals, g, g', lg, L, v0, vs0) => !!(readable_share sh /\
      readable_share shi /\ isptr version /\ Forall isptr locs /\ Zlength locs = size /\
-     Forall repable_signed vals /\ Z.even v0 = true /\ Zlength vs0 = size) &&
+     Forall repable_signed vals /\ Z.even v0 = true /\ Zlength vs0 = size /\ log_latest L v0 vs0) &&
    data_at sh tnode (version, locs) n * data_at shi (tarray tint size) (map (fun x => vint x) vals) input *
-   protocol_W version g g' v0 Z.le (version_T locs g lg lg') * fold_right sepcon emp (map (fun i =>
-     EX log : _, !!(log_latest log v0 (Znth i vs0 0)) &&
-       protocol_W (Znth i locs Vundef) (Znth i lg Vundef) (Znth i lg' Vundef) log log_incl (data_T g))
-     (upto (Z.to_nat size))))
-  (fun _ '(n, input, sh, shi, version, locs, vals, g, g', lg, lg', v0, vs0) '(v, vs) =>
-   node_state v vs version locs g g' lg lg')
+   node_state_W L version locs g lg * ghost (gsh2, L) g')
+  (fun _ '(n, input, sh, shi, version, locs, vals, g, g', lg, L, v0, vs0) L' =>
+   node_state L' version locs g lg * ghost (gsh1, L') g')
   tt []
-  (fun _ '(n, input, sh, shi, version, locs, vals, g, g', lg, lg', v0, vs0) '(v, vs) _ =>
+  (fun _ '(n, input, sh, shi, version, locs, vals, g, g', lg, L, v0, vs0) _ _ =>
    data_at sh tnode (version, locs) n * data_at shi (tarray tint size) (map (fun x => vint x) vals) input *
-   protocol_W version g g' (v0 + 2) Z.le (version_T locs g lg lg') * fold_right sepcon emp (map (fun i =>
-     EX log : _, !!(log_latest log (v0 + 2) (Znth i vals 0)) &&
-       protocol_W (Znth i locs Vundef) (Znth i lg Vundef) (Znth i lg' Vundef) log log_incl (data_T g))
-     (upto (Z.to_nat size))))
-  (fun _ '(n, input, sh, shi, version, locs, vals, g, g', lg, lg', v0, vs0) '(v, vs) _ =>
-   (* !!(v = v0 /\ vs = vs0) && *) node_state (v0 + 2) vals version locs g g' lg lg')
+   node_state_W (map_upd L (v0 + 2) vals) version locs g lg * ghost (gsh2, map_upd L (v0 + 2) vals) g')
+  (fun _ '(n, input, sh, shi, version, locs, vals, g, g', lg, L, v0, vs0) _ _ =>
+   node_state (map_upd L (v0 + 2) vals) version locs g lg * ghost (gsh1, map_upd L (v0 + 2) vals) g')
   _ _ _ _ _ _.
-(* We can prove the stronger postcondition, but the writer doesn't really care what it overwrites. *)
 Next Obligation.
 Proof.
   intros ?? w; decompose [prod] w; auto.
@@ -129,56 +174,100 @@ Proof.
   intros ?? w; decompose [prod] w; auto.
 Qed.
 
-(* The state we've read by the end may be older than the state in the invariant, so we need a history to get
-   anything useful out of the read. *)
-(* On the one hand, it seems like we should be able to know we've gotten the most recent version. On the other
-   hand, that leads directly to SC issues if extended to multiple locations. *)
-Program Definition read_spec := DECLARE _read atomic_spec
-  (ConstType (val * val * share * share * val * list val * val * val * list val * list val * Z * list Z))
-  (0, []) [(_n, tptr tnode); (_out, tptr tint)] tvoid
-  [fun _ '(n, out, sh, shi, version, locs, g, g', lg, lg', v0, vs0) => temp _n n;
-   fun _ '(n, out, sh, shi, version, locs, g, g', lg, lg', v0, vs0) => temp _out out]
-  (fun _ '(n, out, sh, shi, version, locs, g, g', lg, lg', v0, vs0) => !!(readable_share sh /\
-     writable_share shi /\ isptr version /\ Forall isptr locs /\ Zlength locs = size /\ Zlength vs0 = size /\
-     Z.even v0 = true) &&
-   data_at sh tnode (version, locs) n * data_at_ shi (tarray tint size) out *
-   node_state v0 vs0 version locs g g' lg lg')
-  (fun _ '(n, out, sh, shi, version, locs, g, g', lg, lg', v0, vs0) '(v, vs) =>
-   node_state v vs version locs g g' lg lg')
+Definition make_node_spec := DECLARE _make_node
+  WITH u : unit
+  PRE [ ]
+    PROP ()
+    LOCAL ()
+    SEP ()
+  POST [ tptr tnode ]
+   EX n : val, EX version : val, EX locs : list val, EX g : val, EX lg : list val,
+    PROP (isptr version; Forall isptr locs; Zlength locs = size)
+    LOCAL (temp ret_temp n)
+    SEP (data_at Tsh tnode (version, locs) n; malloc_token Tsh (sizeof tnode) n;
+         malloc_token Tsh (sizeof tint) version; fold_right sepcon emp (map (malloc_token Tsh (sizeof tint)) locs);
+         node_state_W (singleton 0 (repeat 0 (Z.to_nat size))) version locs g lg).
+
+Definition writer_spec := DECLARE _writer
+  WITH n : val, sh : share, v : Z, vs : list Z, L : Z -> option (list Z), version : val, locs : list val,
+       g : val, g' : val, lg : list val
+  PRE [ _n OF tptr tvoid ]
+    PROP (readable_share sh; isptr version; Forall isptr locs; Zlength locs = size; Z.even v = true;
+          Zlength vs = size; log_latest L v vs)
+    LOCAL (temp _n n)
+    SEP (data_at sh tnode (version, locs) n; node_state_W L version locs g lg; ghost (gsh2, L) g')
+  POST [ tptr tvoid ]
+   EX L' : _,
+    PROP (L' = map_upd_list L (map (fun i => (v + (2 * (i + 1)), repeat (i + 1) (Z.to_nat size)))%Z (upto 3)))
+    LOCAL ()
+    SEP (data_at sh tnode (version, locs) n; node_state_W L' version locs g lg; ghost (gsh2, L') g').
+
+(*Definition reader_spec := DECLARE _reader
+  WITH n : val, sh : share, version : val, locs : list val, g : val, g' : val,
+       lg : list val, lg' : list val, gh : val, gsh : share
+  PRE [ _n OF tptr tvoid ]
+    PROP (readable_share sh; isptr version; Forall isptr locs; Zlength locs = size; gsh <> Share.bot)
+    LOCAL (temp _n n)
+    SEP (data_at sh tnode (version, locs) n; ghost_hist gsh ([] : hist) gh;
+         invariant (node_inv gh version locs g g' lg lg'))
+  POST [ tptr tvoid ]
+   EX h : hist,
+    PROP (exists v vs, add_events [] [HRead v vs] h)
+    LOCAL ()
+    SEP (data_at sh tnode (version, locs) n; ghost_hist gsh h gh;
+         invariant (node_inv gh version locs g g' lg lg')).*)
+
+(* We can't keep an interleaved history of reads and writes, but we can know that each read got a value
+   that was at some point in the history. *)
+(*Program Definition reader_spec := DECLARE _reader atomic_spec
+  (ConstType (val * share * val * list val * val * val * list val * list val * val * share))
+  tt [(_n, tptr tvoid)] (tptr tvoid)
+  [fun _ '(n, sh, version, locs, g, g', lg, lg', gh, gsh) => temp _n n]
+  (fun _ '(n, sh, version, locs, g, g', lg, lg', gh, gsh) => !!(readable_share sh /\ isptr version /\
+   Forall isptr locs /\ Zlength locs = size /\ gsh <> Share.bot) && data_at sh tnode (version, locs) n)
+  (fun _ '(n, sh, version, locs, g, g', lg, lg', gh, gsh) _ => node_inv gh version locs g g' lg lg')
   (0, []) []
-  (fun _ '(n, out, sh, shi, version, locs, g, g', lg, lg', v0, vs0) '(v, vs) '(v', vals) =>
-   data_at sh tnode (version, locs) n * data_at shi (tarray tint size) (map (fun x => vint x) vals) out *
-   node_state v' vals version locs g g' lg lg')
-  (fun _ '(n, out, sh, shi, version, locs, g, g', lg, lg', v0, vs0) '(v, vs) '(v', vals) =>
-   node_state v vs version locs g g' lg lg' * node_state v' vals version locs g g' lg lg')
-  _ _ _ _ _ _.
-(* We can prove the stronger postcondition, but the writer doesn't really care what it overwrites. *)
-Next Obligation.
-Proof.
-  intros ?? w; decompose [prod] w; auto.
-Qed.
-Next Obligation.
-Proof.
-  intros ?? w; decompose [prod] w; auto.
-Qed.
-Next Obligation.
-Proof.
-  intros ?? w; decompose [prod] w; auto.
-Qed.
-Next Obligation.
-Proof.
-  intros ?? w; decompose [prod] w; auto.
-Qed.
-Next Obligation.
-Proof.
-  intros ?? w; decompose [prod] w; auto.
-Qed.
-Next Obligation.
-Proof.
-  intros ?? w; decompose [prod] w; auto.
-Qed.
+  (fun _ '(n, sh, version, locs, g, g', lg, lg', gh, gsh) _ _ => data_at sh tnode (version, locs) n)
+  (fun _ '(n, sh, version, locs, g, g', lg, lg', gh, gsh) _ '(v1, vs1) =>
+   EX v : Z, EX vs : list Z, node_state v vs version locs g g' lg lg' * EX hr : _,
+     !!(apply_hist (0, repeat 0 (Z.to_nat size)) hr = Some (v, vs) /\ In (HWrite v1 vs1) hr) && ghost_ref hr gh)
+  _ _ _ _ _ _. (* We could encapsulate this with another argument to node_inv, a known sublist of hr. *)*)
 
-Definition Gprog : funspecs := ltac:(with_library prog [load_acq_spec; store_rel_spec; read_spec; write_spec]).
+Definition reader_spec := DECLARE _reader
+  WITH n : val, sh : share, v : Z, vs : list Z, L : Z -> option (list Z), version : val, locs : list val,
+       g : val, g' : val, lg : list val
+  PRE [ _n OF tptr tvoid ]
+    PROP (readable_share sh; isptr version; Forall isptr locs; Zlength locs = size; Z.even v = true;
+          log_latest L v vs)
+    LOCAL (temp _n n)
+    SEP (data_at sh tnode (version, locs) n; node_state L version locs g lg * ghost_snap )
+  POST [ tptr tvoid ]
+   EX v' : Z, EX vs' : list Z,
+    PROP (v <= v'; v' = v -> vs' = vs)
+    LOCAL ()
+    SEP (data_at sh tnode (version, locs) n; node_state (map_upd L v' vs') version locs g g' lg lg').
+(* And combining this node_state with a node_state_W will guarantee that (v', vs') is in the full log. *)
+
+Definition Gprog : funspecs := ltac:(with_library prog [surely_malloc_spec; load_acq_spec; store_rel_spec;
+  read_spec; write_spec; make_node_spec; writer_spec; reader_spec]).
+
+Lemma body_surely_malloc: semax_body Vprog Gprog f_surely_malloc surely_malloc_spec.
+Proof.
+  start_function.
+  forward_call n.
+  Intros p.
+  forward_if
+  (PROP ( )
+   LOCAL (temp _p p)
+   SEP (malloc_token Tsh n p * memory_block Tsh n p)).
+  - if_tac; entailer!.
+  - forward_call tt.
+    contradiction.
+  - if_tac.
+    + forward. subst p. discriminate.
+    + Intros. forward. entailer!.
+  - forward. Exists p; entailer!.
+Qed.
 
 Lemma land_1 : forall i, Z.land i 1 = i mod 2.
 Proof.
@@ -186,851 +275,37 @@ Proof.
 Qed.
 
 Existing Instance max_PCM.
+Existing Instance max_order.
+Existing Instance fmap_PCM.
+Existing Instance fmap_order.
 
-(* up *)
-Lemma Znth_repeat' : forall {A} (d x : A) n i, 0 <= i < Z.of_nat n -> Znth i (repeat x n) d = x.
-Proof.
-  induction n; intros; [simpl in *; omega|].
-  rewrite Nat2Z.inj_succ in H; simpl.
-  destruct (eq_dec i 0).
-  - subst; apply Znth_0_cons.
-  - rewrite Znth_pos_cons by omega; apply IHn; omega.
-Qed.
-
-(* automation for dependent funspecs *)
-Definition call_setup2'
-  (cs: compspecs) Qtemp Qvar a Delta P Q R  
-   argsig retty cc ts (A: rmaps.TypeTree)  Pre Post NEPre NEPost
-  (bl: list expr) (vl : list val)
-  (Qactuals : PTree.t _)
-  (witness: functors.MixVariantFunctor._functor (rmaps.dependent_type_functor_rec ts A) mpred)
-  (Frame: list mpred)
-  (Ppre: list Prop) (Qpre : list localdef) (Rpre: list mpred)
-  (Qpre_temp : PTree.t _) (Qpre_var: PTree.t vardesc) :=
- call_setup1 cs Qtemp Qvar a Delta P Q R argsig retty cc A Pre Post NEPre NEPost bl vl Qactuals /\
-  Pre ts witness = PROPx Ppre (LOCALx Qpre (SEPx Rpre)) /\
-  local2ptree Qpre = (Qpre_temp, Qpre_var, nil, nil) /\
-  ENTAIL Delta, PROPx P (LOCALx Q (SEPx R))
-           |-- !! Forall (check_one_temp_spec Qactuals) (PTree.elements Qpre_temp) /\
-  ENTAIL Delta, PROPx P (LOCALx Q (SEPx R))
-           |-- !! Forall (check_one_var_spec Qvar) (PTree.elements Qpre_var) /\
-  fold_right_sepcon R |-- fold_right_sepcon Rpre * fold_right_sepcon Frame.
-
-Lemma call_setup2'_i:
- forall  (cs: compspecs) Qtemp Qvar a Delta P Q R  
-   argsig retty cc ts (A: rmaps.TypeTree) Pre Post NEPre NEPost
-  (bl: list expr) (vl : list val)
-  (Qactuals : PTree.t _)
-  (SETUP1: call_setup1 cs Qtemp Qvar a Delta P Q R argsig retty cc A Pre Post NEPre NEPost bl vl Qactuals)
-  (witness': functors.MixVariantFunctor._functor (rmaps.dependent_type_functor_rec ts A) mpred)
-  (Frame: list mpred)
-  (Ppre: list Prop) (Qpre : list localdef) (Rpre: list mpred)
-  (Qpre_temp : PTree.t _) (Qpre_var: PTree.t vardesc),
-  Pre ts witness' = PROPx Ppre (LOCALx Qpre (SEPx Rpre)) ->
-  local2ptree Qpre = (Qpre_temp, Qpre_var, nil, nil) ->
-  ENTAIL Delta, PROPx P (LOCALx Q (SEPx R))
-           |-- !! Forall (check_one_temp_spec Qactuals) (PTree.elements Qpre_temp) ->
-  ENTAIL Delta, PROPx P (LOCALx Q (SEPx R))
-           |-- !! Forall (check_one_var_spec Qvar) (PTree.elements Qpre_var)  ->
-  fold_right_sepcon R |-- fold_right_sepcon Rpre * fold_right_sepcon Frame ->
-  call_setup2' cs Qtemp Qvar a Delta P Q R argsig retty cc ts A Pre Post NEPre NEPost bl vl Qactuals
-      witness' Frame Ppre Qpre Rpre Qpre_temp Qpre_var.
-Proof.
- intros. split. auto. repeat split; auto.
-Qed.
-
-Ltac check_witness_type' ts A witness :=
-  (unify A (rmaps.ConstType Ridiculous); (* because [is_evar A] doesn't seem to work *)
-             elimtype False)
- ||
- let TA := constr:(functors.MixVariantFunctor._functor
-     (rmaps.dependent_type_functor_rec ts A) mpred) in
-  let TA' := eval cbv 
-     [functors.MixVariantFunctor._functor
-      functors.MixVariantFunctorGenerator.fpair
-      functors.MixVariantFunctorGenerator.fconst
-      functors.MixVariantFunctorGenerator.fidentity
-      rmaps.dependent_type_functor_rec
-      functors.GeneralFunctorGenerator.CovariantBiFunctor_MixVariantFunctor_compose
-      functors.CovariantFunctorGenerator.fconst
-      functors.CovariantFunctorGenerator.fidentity
-      functors.CovariantBiFunctor._functor
-      functors.CovariantBiFunctorGenerator.Fpair
-      functors.GeneralFunctorGenerator.CovariantFunctor_MixVariantFunctor
-      functors.CovariantFunctor._functor
-      functors.MixVariantFunctor.fmap
-      ] in TA
- in let TA'' := eval simpl in TA'
-  in match type of witness with ?T => 
-       unify T TA''
-      + (fail "Type of witness does not match type required by funspec WITH clause.
-Witness value: " witness "
-Witness type: " T "
-Funspec type: " TA'')
-     end.
-
-Ltac prove_call_setup' ts witness :=
- prove_call_setup1;
- [ .. | 
- match goal with |- call_setup1 _ _ _ _ _ _ _ _ _ _ _ ?A _ _ _ _ _ _ _ -> _ =>
-      check_witness_type' ts A witness
- end;
- let H := fresh in
- intro H;
- let Frame := fresh "Frame" in evar (Frame: list mpred);
- exploit (call_setup2'_i _ _ _ _ _ _ _ _ _ _ _ ts _ _ _ _ _ _ _ _ H witness Frame); clear H;
- simpl functors.MixVariantFunctor._functor;
- [ reflexivity
- | check_prove_local2ptree
- | Forall_pTree_from_elements
- | Forall_pTree_from_elements
- | unfold fold_right_sepcon at 1 2; cancel_for_forward_call
- | 
- ]].
-
-Lemma semax_call_aux55:
- forall (cs: compspecs) (Qtemp: PTree.t val) (Qvar: PTree.t vardesc) (a: expr)
-     Delta P Q R argsig retty cc ts A Pre Post NEPre NEPost 
-    witness Frame bl Ppre Qpre Rpre Qactuals Qpre_temp Qpre_var vl
- (PTREE : local2ptree Q = (Qtemp, Qvar, nil, nil))
- (TC0 : ENTAIL Delta, PROPx P (LOCALx Q (SEPx R)) |-- tc_expr Delta a)
- (TC1 : ENTAIL Delta, PROPx P (LOCALx Q (SEPx R))
-             |-- tc_exprlist Delta (argtypes argsig) bl)
- (MSUBST : force_list (map (msubst_eval_expr Qtemp Qvar)
-              (explicit_cast_exprlist (argtypes argsig) bl)) = Some vl)
- (PTREE'' : pTree_from_elements (combine (var_names argsig) vl) = Qactuals)
- (PRE1 : Pre ts witness = PROPx Ppre (LOCALx Qpre (SEPx Rpre)))
- (PTREE' : local2ptree Qpre = (Qpre_temp, Qpre_var, nil, nil)) 
- (CHECKTEMP : ENTAIL Delta, PROPx P (LOCALx Q (SEPx R))
-            |-- !! Forall (check_one_temp_spec Qactuals)
-                     (PTree.elements Qpre_temp))
- (CHECKVAR : ENTAIL Delta, PROPx P (LOCALx Q (SEPx R))
-           |-- !! Forall (check_one_var_spec Qvar) (PTree.elements Qpre_var))
- (FRAME : fold_right_sepcon R
-           |-- fold_right_sepcon Rpre * fold_right_sepcon Frame)
- (PPRE : fold_right_and True Ppre),
-ENTAIL Delta,
-(EX v : val,
- lift0 (func_ptr (mk_funspec (argsig, retty) cc A Pre Post NEPre NEPost) v) &&
- local (` (eq v) (eval_expr a))) && PROPx P (LOCALx Q (SEPx R))
-|-- tc_expr Delta a && tc_exprlist Delta (argtypes argsig) bl &&
-    (` (Pre ts witness)
-       (make_args' (argsig, retty) (eval_exprlist (argtypes argsig) bl)) *
-     ` (func_ptr' (mk_funspec (argsig, retty) cc A Pre Post NEPre NEPost))
-       (eval_expr a) * PROPx P (LOCALx Q (SEPx Frame))).
-Proof.
-intros.
-rewrite !exp_andp1. Intros v.
-repeat apply andp_right; auto.
-eapply derives_trans; [apply andp_derives; [apply derives_refl | apply andp_left2; apply derives_refl ] | auto].
-eapply derives_trans; [apply andp_derives; [apply derives_refl | apply andp_left2; apply derives_refl ] | auto].
-(*
-normalize.
-assert (H0 := @msubst_eval_expr_eq cs P Qtemp Qvar nil R a v).
-assert (H1 := local2ptree_soundness P Q R Qtemp Qvar nil nil PTREE).
-simpl app in H1. rewrite <- H1 in H0. apply H0 in EVAL. 
-clear H0 H1.
-*)
-rewrite PRE1.
-match goal with |- _ |-- ?A * ?B * ?C => pull_right B end.
-rewrite sepcon_comm.
-rewrite func_ptr'_func_ptr_lifted.
-apply ENTAIL_trans with
- (`(func_ptr (mk_funspec (argsig, retty) cc A Pre Post NEPre NEPost)) (eval_expr a) &&
-      PROPx P (LOCALx Q (SEPx R))).
-apply andp_left2.
-apply andp_right; [  | apply andp_left2; auto].
-apply andp_left1.
-intro rho; unfold_lift; unfold local, lift0, lift1; simpl. normalize.
-apply andp_right.
-apply andp_left2; apply andp_left1; auto.
-eapply derives_trans;[ apply andp_derives; [apply derives_refl | apply andp_left2; apply derives_refl] |].
- match goal with |- ?D && PROPx ?A ?B |-- ?C =>
-  apply derives_trans with (D && PROPx ((length (argtypes argsig) = length bl) :: A) B);
-    [ rewrite <- insert_prop | ]
- end.
- apply andp_right; [apply andp_left1; auto | ].
- apply andp_right; [| apply andp_left2; auto].
- eapply derives_trans; [apply TC1 | ].
- clear. go_lowerx.
- unfold tc_exprlist.
- revert bl; induction (argtypes argsig); destruct bl;
-   simpl; try apply @FF_left.
- apply prop_right; auto.
- repeat rewrite denote_tc_assert_andp. apply andp_left2.
- eapply derives_trans; [ apply IHl | ]. normalize.
-apply derives_extract_PROP; intro LEN.
-subst Qactuals. 
-clear - PTREE LEN PTREE' MSUBST CHECKVAR FRAME PPRE CHECKTEMP.
- progress (autorewrite with norm1 norm2); normalize.
- eapply derives_trans.
- apply andp_right. apply andp_right. apply CHECKVAR. apply CHECKTEMP. apply derives_refl.
- rewrite andp_assoc. apply derives_extract_prop; intro CVAR.
- apply derives_extract_prop; intro CTEMP.
- clear CHECKTEMP CHECKVAR.
-rewrite PROP_combine.
-rewrite (andp_comm (local (fold_right _ _ _))).
-apply andp_right.
-+
-apply andp_right.
-apply andp_left2.
-apply andp_left1.
-rewrite fold_right_and_app_low.
-apply prop_derives; intros; split; auto.
- clear - PPRE.
- revert PPRE; induction Ppre; simpl; intuition.
-apply andp_left2.
-apply andp_left2.
-apply andp_derives.
-apply derives_refl.
-intro rho; unfold SEPx.
- rewrite fold_right_sepcon_app.
- assumption.
-+
- apply (local2ptree_soundness P _ R) in PTREE.
- simpl app in PTREE.
- apply msubst_eval_exprlist_eq with (P:=P)(R:=R)(Q:=nil) in MSUBST.
- rewrite PTREE.
- intro rho.
- unfold local, lift1. unfold_lift. simpl.
- apply andp_left2.
- eapply derives_trans. apply andp_right. apply MSUBST. apply derives_refl.
- clear MSUBST.
- apply (local2ptree_soundness nil _ (TT::nil)) in PTREE'.
- simpl app in PTREE'.
- rewrite !isolate_LOCAL_lem1 in PTREE'.
- unfold local at 1, lift1.
- simpl.
- apply derives_extract_prop; intro. unfold_lift in H. subst vl.
- unfold PROPx, LOCALx, SEPx. simpl.
-apply andp_left2. apply andp_left1.
- assert (LEN': length (var_names argsig) = length (eval_exprlist (argtypes argsig) bl rho)).
- clear - LEN.
-  revert bl LEN; induction argsig as [ | [? ?]]; destruct bl;
-    simpl; intros; auto.
- inv LEN.
- forget (argtypes argsig) as tys.
- cut (local (fold_right `and `True (map locald_denote (LocalD Qtemp Qvar nil))) rho |--
-            `(local (fold_right `and `True (map locald_denote Qpre)))
-               (fun rho => (make_args (var_names argsig) (eval_exprlist tys bl rho) rho)) rho).
- intro. eapply derives_trans; [apply H  |].
- unfold make_args'. simpl @fst. change (map fst argsig) with (var_names argsig).
- clear.  unfold_lift. unfold local, lift1. apply prop_derives.
- induction Qpre; simpl; auto.  intros [? ?]. split; auto.
- rewrite PTREE'. clear PTREE' Qpre.
- apply prop_derives; intro. forget (var_names argsig) as fl.
- forget (eval_exprlist tys bl rho) as vl.
- eapply check_specs_lemma; try eassumption.
-Qed.
-
-Lemma semax_call_id00_wow:
- forall  
-  (cs: compspecs) Qtemp Qvar a Delta P Q R  
-   argsig retty cc ts (A: rmaps.TypeTree)  Pre Post NEPre NEPost
-   (witness: functors.MixVariantFunctor._functor (rmaps.dependent_type_functor_rec ts A) mpred) 
-   (Frame: list mpred)
-   (bl: list expr)
-   (Ppre: list Prop) (Qpre : list localdef) (Rpre: list mpred)
-   (Qactuals Qpre_temp : PTree.t _) (Qpre_var: PTree.t vardesc)
-   (vl : list val)
-   (SETUP: call_setup2' cs Qtemp Qvar a Delta P Q R argsig retty cc ts A Pre Post NEPre NEPost bl vl Qactuals
-      witness Frame Ppre Qpre Rpre Qpre_temp Qpre_var)
-  Espec 
-             (Post2: environ -> mpred)
-             (B: Type)
-             (Ppost: B -> list Prop)
-             (Rpost: B -> list mpred)
-   (RETTY: retty = Tvoid)
-   (POST1: Post ts witness = (EX vret:B, PROPx (Ppost vret) (LOCALx nil (SEPx (Rpost vret)))))
-   (POST2: Post2 = EX vret:B, PROPx (P++ Ppost vret ) (LOCALx Q
-             (SEPx (Rpost vret ++ Frame))))
-   (PPRE: fold_right_and True Ppre),
-   @semax cs Espec Delta (PROPx P (LOCALx Q (SEPx R)))
-    (Scall None a bl)
-    (normal_ret_assert Post2).
-Proof.
-intros.
-destruct SETUP as [[PTREE [SPEC [ATY [TC0 [TC1 [MSUBST PTREE'']]]]]] 
-                            [PRE1 [PTREE' [CHECKTEMP [CHECKVAR FRAME]]]]].
-apply SPEC. clear SPEC.
-eapply semax_pre_post; [ | |
-   apply (@semax_call0 Espec cs Delta A Pre Post NEPre NEPost 
-              ts witness argsig retty cc a bl P Q Frame)].
-*
-eapply semax_call_aux55; eauto.
-*
- subst.
- clear CHECKVAR CHECKTEMP TC1 PRE1 PPRE.
- intros.
- unfold normal_ret_assert. normalize.
- simpl exit_tycon. rewrite POST1; clear POST1.
- unfold ifvoid.
- go_lowerx. normalize.
- apply exp_right with x.
- apply andp_right.
- apply prop_right.
- split; auto.
- normalize.
- rewrite fold_right_and_app_low.
- rewrite prop_true_andp by (split; auto).
- rewrite fold_right_sepcon_app. auto.
-*
-assumption.
-Qed.
-
-Lemma semax_call_id1_wow:
- forall  
-  (cs: compspecs) Qtemp Qvar a Delta P Q R  
-   argsig retty cc ts (A: rmaps.TypeTree)  Pre Post NEPre NEPost
-   (witness: functors.MixVariantFunctor._functor (rmaps.dependent_type_functor_rec ts A) mpred) 
-   (Frame: list mpred)
-   (bl: list expr)
-   (Ppre: list Prop) (Qpre : list localdef) (Rpre: list mpred)
-   (Qactuals Qpre_temp : PTree.t _) (Qpre_var: PTree.t vardesc)
-   (vl : list val)
-   (SETUP: call_setup2' cs Qtemp Qvar a Delta P Q R argsig retty cc ts A Pre Post NEPre NEPost bl vl Qactuals
-      witness Frame Ppre Qpre Rpre Qpre_temp Qpre_var)
-   ret (Post2: environ -> mpred)  (Qnew: list localdef)
-    (B: Type) (Ppost: B -> list Prop) (F: B -> val) (Rpost: B -> list mpred) Espec
-   (TYret: typeof_temp Delta ret = Some retty)
-   (OKretty: check_retty retty)
-   (POST1: Post ts witness = EX vret:B, PROPx (Ppost vret)
-                              (LOCALx (temp ret_temp (F vret) :: nil)
-                              (SEPx (Rpost vret))))
-   (DELETE: remove_localdef_temp ret Q = Qnew)
-   (H0: Post2 = EX vret:B, PROPx (P++ Ppost vret) (LOCALx (temp ret (F vret) :: Qnew)
-             (SEPx (Rpost vret ++ Frame))))
-   (PPRE: fold_right_and True Ppre),
-   @semax cs Espec Delta (PROPx P (LOCALx Q (SEPx R)))
-    (Scall (Some ret) a bl)
-    (normal_ret_assert Post2).
-Proof.
-intros. 
-destruct SETUP as [[PTREE [SPEC [ATY [TC0 [TC1 [MSUBST PTREE'']]]]]] 
-                            [PRE1 [PTREE' [CHECKTEMP [CHECKVAR FRAME]]]]].
-apply SPEC. clear SPEC.
-eapply semax_pre_post; [ | |
-   apply (@semax_call1 Espec cs Delta A Pre Post NEPre NEPost 
-              ts witness ret argsig retty cc a bl P Q Frame)];
- [ | 
- | assumption
- | clear - OKretty; destruct retty; inv OKretty; apply I
- | hnf; clear - TYret; unfold typeof_temp in TYret;
-      destruct ((temp_types Delta) ! ret) as [[? ?] | ]; inv TYret; auto
- ].
-*
-eapply semax_call_aux55; eauto.
-*
- subst.
- clear CHECKVAR CHECKTEMP TC1 PRE1 PPRE.
- intros.
- unfold normal_ret_assert. normalize.
- simpl exit_tycon. rewrite POST1; clear POST1.
- apply derives_trans with
-   (EX  vret : B,
-    `(PROPx (Ppost vret)
-     (LOCAL  (temp ret_temp (F vret))
-      (SEPx (Rpost vret))))%assert (get_result1 ret)
-     * (local (tc_environ (initialized ret Delta)) && PROPx P (LOCALx (remove_localdef_temp ret Q) (SEPx Frame)))).
- clear.
- go_lowerx. normalize. apply exp_right with x; normalize.
- apply exp_left; intro vret. apply exp_right with vret.
- normalize.
- progress (autorewrite with norm1 norm2); normalize.
- rewrite PROP_combine.
- unfold fold_right.
- go_lowerx.
- repeat apply andp_right; try apply prop_right; auto.
- rewrite !fold_right_and_app_low.
- rewrite !fold_right_and_app_low in H2. destruct H2; split; auto.
-Qed.
-
-Lemma semax_call_id1_x_wow:
- forall  (cs: compspecs) Qtemp Qvar a Delta P Q R  
-   argsig retty' cc ts (A: rmaps.TypeTree)  Pre Post NEPre NEPost
-   (witness: functors.MixVariantFunctor._functor (rmaps.dependent_type_functor_rec ts A) mpred) 
-   (Frame: list mpred)
-   (bl: list expr)
-   (Ppre: list Prop) (Qpre : list localdef) (Rpre: list mpred)
-   (Qactuals Qpre_temp : PTree.t _) (Qpre_var: PTree.t vardesc)
-   (vl : list val)
-   (SETUP: call_setup2' cs Qtemp Qvar a Delta P Q R argsig retty' cc ts A Pre Post NEPre NEPost bl vl Qactuals
-      witness Frame Ppre Qpre Rpre Qpre_temp Qpre_var)
-   retty  Espec ret ret'
-             (Post2: environ -> mpred)
-             (Qnew: list localdef)
-             (B: Type)
-             (Ppost: B -> list Prop)
-             (F: B -> val)
-             (Rpost: B -> list mpred)
-   (TYret: typeof_temp Delta ret = Some retty)
-   (RETinit: (temp_types Delta) ! ret' = Some (retty', false))
-   (OKretty: check_retty retty)
-   (OKretty': check_retty retty')
-   (NEUTRAL: is_neutral_cast retty' retty = true)
-   (NEret: ret <> ret')
-   (POST1: Post ts witness = EX vret:B, PROPx (Ppost vret)
-                              (LOCALx (temp ret_temp (F vret) :: nil)
-                              (SEPx (Rpost vret))))
-   (DELETE: remove_localdef_temp ret Q = Qnew)
-   (DELETE' : remove_localdef_temp ret' Q = Q)
-   (H0: Post2 = EX vret:B, PROPx (P++ Ppost vret)
-                   (LOCALx (temp ret (F vret) :: Qnew)
-                    (SEPx (Rpost vret ++ Frame))))
-   (PPRE: fold_right_and True Ppre),
-   @semax cs Espec Delta (PROPx P (LOCALx Q (SEPx R)))
-   (Ssequence (Scall (Some ret') a bl)
-      (Sset ret (Ecast (Etempvar ret' retty') retty)))
-    (normal_ret_assert Post2).
-Proof.
-intros.
-eapply semax_seq'.
-eapply semax_call_id1_wow; try eassumption; auto.
-  unfold typeof_temp; rewrite RETinit; reflexivity.
- simpl update_tycon.
- apply extract_exists_pre; intro vret.
-*
- eapply semax_pre_post;
- [ | | apply semax_set_forward].
- +
- eapply derives_trans; [ | apply now_later ].
- instantiate (1:= (PROPx (P ++ Ppost vret)
-  (LOCALx (temp ret' (F vret) :: Qnew) (SEPx (Rpost vret ++ Frame))))).
- apply andp_right.
- apply andp_right.
- unfold tc_expr.
- unfold typecheck_expr; simpl.
- simpl denote_tc_assert.
- rewrite tycontext.temp_types_same_type'. rewrite RETinit.
- simpl @fst.
- replace ((is_neutral_cast retty' retty' || same_base_type retty' retty')%bool)
-   with true
-  by (clear- OKretty'; destruct retty' as [ | [ | | |] [| ]| [|] | [ | ] |  | | | | ]; try contradiction;
-    reflexivity).
- simpl @snd. cbv iota.
- go_lowerx. simpl.
- apply neutral_isCastResultType; auto.
- unfold tc_temp_id, typecheck_temp_id.
- rewrite <- tycontext.initialized_ne by auto.
- unfold typeof_temp in TYret.
- destruct ((temp_types Delta) ! ret) as [[? ?]  | ]; inversion TYret; clear TYret; try subst t.
- go_lowerx.
- repeat rewrite denote_tc_assert_andp.
- rewrite denote_tc_assert_bool.
- assert (is_neutral_cast (implicit_deref retty) retty = true)
-  by (destruct retty as [ | [ | | |] [| ]| [|] | [ | ] |  | | | | ]; try contradiction; simpl; auto;
-        destruct retty' as [ | [ | | |] [| ]| [|] | [ | ] |  | | | | ]; try contradiction; inv NEUTRAL).
- apply andp_right. apply prop_right; auto.
- apply neutral_isCastResultType; auto.
- go_lowerx. normalize. apply andp_right; auto. apply prop_right.
- subst Qnew; clear - H3. rename H3 into H.
- induction Q; simpl in *; auto.
- destruct H, a; specialize (IHQ H0); try now (simpl; split; auto).
- hnf in H.
- if_tac; simpl; auto.
-+
- intros. subst Post2.
- unfold normal_ret_assert.
- normalize. simpl exit_tycon.
- apply exp_right with vret; normalize.
- autorewrite with subst.
- go_lowerx.
- normalize. apply andp_right; auto.
- apply prop_right; split; auto.
- hnf. rewrite H0; unfold_lift.
- assert (eqb_ident ret ret' = false)
- by (clear - NEret; pose proof (eqb_ident_spec ret ret');
-       destruct (eqb_ident ret ret'); auto;
-      contradiction NEret; intuition).
- rewrite H4 in *. apply Pos.eqb_neq in H4.
-  unfold_lift in H2.
-  rewrite eval_id_other in H2 by auto.
- hnf in H2. rewrite H2.
- assert (tc_val retty' (eval_id ret' rho)).
- eapply tc_eval_id_i; try eassumption.
- rewrite <- initialized_ne by auto.
-  rewrite temp_types_same_type'.
- rewrite RETinit. auto.
- assert (H7 := expr2.neutral_cast_lemma);
-   unfold eval_cast in H7. rewrite H7 by auto.
- unfold eval_id, env_set, Map.get. auto.
- subst Qnew; clear - H3. rename H3 into H.
- induction Q; simpl in *; auto.
- destruct a; try now (destruct H; simpl in *; split; auto).
- if_tac; simpl in *; auto.
- destruct H; split; auto.
- hnf in H|-*; subst.
- rewrite eval_id_other by auto.
- auto.
-Qed.
-
-Lemma semax_call_id1_y_wow:
- forall  (cs: compspecs) Qtemp Qvar a Delta P Q R  
-   argsig retty' cc ts (A: rmaps.TypeTree)  Pre Post NEPre NEPost
-   (witness: functors.MixVariantFunctor._functor (rmaps.dependent_type_functor_rec ts A) mpred) 
-   (Frame: list mpred)
-   (bl: list expr)
-   (Ppre: list Prop) (Qpre : list localdef) (Rpre: list mpred)
-   (Qactuals Qpre_temp : PTree.t _) (Qpre_var: PTree.t vardesc)
-   (vl : list val)
-   (SETUP: call_setup2' cs Qtemp Qvar a Delta P Q R argsig retty' cc ts A Pre Post NEPre NEPost bl vl Qactuals
-      witness Frame Ppre Qpre Rpre Qpre_temp Qpre_var)
-    Espec ret ret' (retty: type) 
-             (Post2: environ -> mpred)
-             (Qnew: list localdef)
-             (B: Type)
-             (Ppost: B -> list Prop)
-             (F: B -> val)
-             (Rpost: B -> list mpred)
-   (TYret: typeof_temp Delta ret = Some retty)
-   (RETinit: (temp_types Delta) ! ret' = Some (retty', false))
-   (OKretty: check_retty retty)
-   (OKretty': check_retty retty')
-   (NEUTRAL: is_neutral_cast retty' retty = true)
-   (NEret: ret <> ret')
-   (POST1: Post ts witness = EX vret:B, PROPx (Ppost vret)
-                              (LOCALx (temp ret_temp (F vret) :: nil)
-                              (SEPx (Rpost vret))))
-   (DELETE: remove_localdef_temp ret Q = Qnew)
-   (DELETE' : remove_localdef_temp ret' Q = Q)
-   (H0: Post2 = EX vret:B, PROPx (P++ Ppost vret)
-                   (LOCALx (temp ret (F vret) :: Qnew)
-                    (SEPx (Rpost vret ++ Frame))))
-   (PPRE: fold_right_and True Ppre),
-   @semax cs Espec Delta (PROPx P (LOCALx Q (SEPx R)))
-   (Ssequence (Scall (Some ret') a bl)
-      (Sset ret (Etempvar ret' retty')))
-    (normal_ret_assert Post2).
-Proof.
-intros.
-eapply semax_seq'.
-eapply semax_call_id1_wow; try eassumption; auto;
-  unfold typeof_temp; rewrite RETinit; reflexivity.
- simpl update_tycon.
- apply extract_exists_pre; intro vret.
-*
- eapply semax_pre_post;
- [ | | apply semax_set_forward].
- +
- eapply derives_trans; [ | apply now_later ].
- instantiate (1:= (PROPx (P ++ Ppost vret)
-  (LOCALx (temp ret' (F vret) :: Qnew) (SEPx (Rpost vret ++ Frame))))).
- apply andp_right.
- apply andp_right.
- unfold tc_expr.
-match goal with |- _ |-- ?A =>
-  set (aa:=A); unfold denote_tc_assert in aa; simpl in aa; subst aa
-end.
- rewrite tycontext.temp_types_same_type'. rewrite RETinit.
- simpl @fst.
- replace ((is_neutral_cast retty' retty' || same_base_type retty' retty')%bool)
-   with true
-  by (clear- OKretty'; destruct retty' as [ | [ | | |] [| ]| [|] | [ | ] |  | | | | ]; try contradiction;
-    reflexivity).
- simpl @snd. cbv iota.
- apply @TT_right.
- unfold tc_temp_id, typecheck_temp_id.
- rewrite <- tycontext.initialized_ne by auto.
- unfold typeof_temp in TYret.
- destruct ((temp_types Delta) ! ret) as [[? ?]  | ]; inversion TYret; clear TYret; try subst t.
- go_lowerx.
- repeat rewrite denote_tc_assert_andp.
- rewrite denote_tc_assert_bool.
- assert (is_neutral_cast (implicit_deref retty') retty = true).
- replace (implicit_deref retty') with retty'
- by (destruct retty' as [ | [ | | |] [| ]| [|] | [ | ] |  | | | | ]; try contradiction; reflexivity).
- auto.
- apply andp_right. apply prop_right; auto.
- apply neutral_isCastResultType; auto.
- go_lowerx. normalize. apply andp_right; auto. apply prop_right.
- subst Qnew; clear - H3. rename H3 into H.
- induction Q; simpl in *; auto.
- destruct H, a; specialize (IHQ H0); try now (simpl; split; auto).
- hnf in H.
- if_tac; simpl; auto.
-+
- intros. subst Post2.
- unfold normal_ret_assert.
- normalize. simpl exit_tycon.
- apply exp_right with vret; normalize.
- autorewrite with subst.
- go_lowerx.
- normalize. apply andp_right; auto.
- apply prop_right; split; auto.
- hnf. rewrite H0; unfold_lift.
- assert (eqb_ident ret ret' = false)
- by (clear - NEret; pose proof (eqb_ident_spec ret ret');
-       destruct (eqb_ident ret ret'); auto;
-      contradiction NEret; intuition).
- rewrite H4 in *.  apply Pos.eqb_neq in H4.
- unfold_lift in H2.
- rewrite eval_id_other in H2 by auto.
- hnf in H2. rewrite H2. auto.
- subst Qnew; clear - H3. rename H3 into H.
- induction Q; simpl in *; auto.
- destruct a; try now (destruct H; simpl in *; split; auto).
- if_tac; simpl in *; auto.
- destruct H; split; auto.
- hnf in H|-*; subst.
- rewrite eval_id_other by auto.
- auto.
-Qed.
-
-Lemma semax_call_id01_wow:
- forall  
-  (cs: compspecs) Qtemp Qvar a Delta P Q R  
-   argsig retty cc ts (A: rmaps.TypeTree)  Pre Post NEPre NEPost
-   (witness: functors.MixVariantFunctor._functor (rmaps.dependent_type_functor_rec ts A) mpred) 
-   (Frame: list mpred)
-   (bl: list expr)
-   (Ppre: list Prop) (Qpre : list localdef) (Rpre: list mpred)
-   (Qactuals Qpre_temp : PTree.t _) (Qpre_var: PTree.t vardesc)
-   (vl : list val)
-   (SETUP: call_setup2' cs Qtemp Qvar a Delta P Q R argsig retty cc ts A Pre Post NEPre NEPost bl vl Qactuals
-      witness Frame Ppre Qpre Rpre Qpre_temp Qpre_var)
-   Espec
-             (Post2: environ -> mpred)
-             (B: Type)
-             (Ppost: B -> list Prop)
-             (F: B -> val)
-             (Rpost: B -> list mpred)
-   (_: check_retty retty)
-         (* this hypothesis is not needed for soundness, just for selectivity *)
-   (POST1: Post ts witness = EX vret:B, PROPx (Ppost vret)
-                              (LOCALx (temp ret_temp (F vret) :: nil)
-                              (SEPx (Rpost vret))))
-   (POST2: Post2 = EX vret:B, PROPx (P++ Ppost vret) (LOCALx Q
-             (SEPx (Rpost vret ++ Frame))))
-   (PPRE: fold_right_and True Ppre),
-   @semax cs Espec Delta (PROPx P (LOCALx Q (SEPx R)))
-    (Scall None a bl)
-    (normal_ret_assert Post2).
-Proof.
-intros.
-destruct SETUP as [[PTREE [SPEC [ATY [TC0 [TC1 [MSUBST PTREE'']]]]]] 
-                            [PRE1 [PTREE' [CHECKTEMP [CHECKVAR FRAME]]]]].
-apply SPEC. clear SPEC.
-eapply semax_pre_post;
-   [ |
-   | apply semax_call0 with (A:= A) (ts := ts)(x:=witness) (P:=P)(Q:=Q)(NEPre :=NEPre) (NEPost := NEPost)(R := Frame)
-   ];
-   try eassumption.
-*
-eapply semax_call_aux55; eauto.
-*
- subst.
- clear CHECKVAR CHECKTEMP TC1 PRE1 PPRE.
- intros.
- unfold normal_ret_assert. normalize.
- simpl exit_tycon. rewrite POST1; clear POST1.
- match goal with |- context [ifvoid retty ?A ?B] =>
-   replace (ifvoid retty A B) with B
-   by (destruct retty; try contradiction; auto)
- end.
- go_lowerx. normalize. apply exp_right with x0; normalize.
- apply andp_right; auto.
- apply prop_right.
- rewrite fold_right_and_app_low. split; auto.
- rename x0 into vret.
- clear.
- rewrite fold_right_sepcon_app. auto.
-Qed.
-
-Ltac  forward_call_id1_wow' := 
-let H := fresh in intro H;
-eapply (semax_call_id1_wow _ _ _ _ _ _ _ _ _ _ _ _ _ _ _ _ _ _ _ _ _ _ _ _ _ _ _ H);
- clear H;
- lazymatch goal with Frame := _ : list mpred |- _ => try clear Frame end;
- [check_result_type
- |apply Logic.I
- | cbv beta iota zeta; unfold_post; extensionality rho;
-   repeat rewrite exp_uncurry;
-   try rewrite no_post_exists; repeat rewrite exp_unfold;
-   first [apply exp_congr; intros ?vret; reflexivity
-           | give_EX_warning
-           ]
- | prove_delete_temp
- | unify_postcondition_exps
- | unfold fold_right_and; repeat rewrite and_True; auto
- ].
-
-Ltac forward_call_id1_x_wow' :=
-let H := fresh in intro H;
-eapply (semax_call_id1_x_wow _ _ _ _ _ _ _ _ _ _ _ _ _ _ _ _ _ _ _ _ _ _ _ _ _ _ _ H); 
- clear H;
- lazymatch goal with Frame := _ : list mpred |- _ => try clear Frame end;
- [ check_result_type | check_result_type
- | apply Coq.Init.Logic.I | apply Coq.Init.Logic.I | reflexivity
- | (clear; let H := fresh in intro H; inversion H)
- | cbv beta iota zeta; unfold_post; extensionality rho;
-   repeat rewrite exp_uncurry;
-   try rewrite no_post_exists; repeat rewrite exp_unfold;
-   first [apply exp_congr; intros ?vret; reflexivity
-           | give_EX_warning
-           ]
- | prove_delete_temp
- | prove_delete_temp
- | unify_postcondition_exps
- | unfold fold_right_and; repeat rewrite and_True; auto
- ].
-
-
-Ltac forward_call_id1_y_wow' :=
-let H := fresh in intro H;
-eapply (semax_call_id1_y_wow _ _ _ _ _ _ _ _ _ _ _ _ _ _ _ _ _ _ _ _ _ _ _ _ _ _ _ H); 
- clear H;
- lazymatch goal with Frame := _ : list mpred |- _ => try clear Frame end;
- [ check_result_type | check_result_type
- | apply Coq.Init.Logic.I | apply Coq.Init.Logic.I | reflexivity
- | (clear; let H := fresh in intro H; inversion H)
- | cbv beta iota zeta; unfold_post; extensionality rho;
-   repeat rewrite exp_uncurry;
-   try rewrite no_post_exists; repeat rewrite exp_unfold;
-   first [apply exp_congr; intros ?vret; reflexivity
-           | give_EX_warning
-           ]
- | prove_delete_temp
- | prove_delete_temp
- | unify_postcondition_exps
- | unfold fold_right_and; repeat rewrite and_True; auto
- ].
-
-Ltac forward_call_id01_wow' :=
-let H := fresh in intro H;
-eapply (semax_call_id01_wow _ _ _ _ _ _ _ _ _ _ _ _ _ _ _ _ _ _ _ _ _ _ _ _ _ _ _ H); 
- clear H;
- lazymatch goal with Frame := _ : list mpred |- _ => try clear Frame end;
- [ apply Coq.Init.Logic.I 
- | cbv beta iota zeta; unfold_post; extensionality rho;
-   repeat rewrite exp_uncurry;
-   try rewrite no_post_exists; repeat rewrite exp_unfold;
-   first [apply exp_congr; intros ?vret; reflexivity
-           | give_EX_warning
-           ]
- | unify_postcondition_exps
- | unfold fold_right_and; repeat rewrite and_True; auto
- ].
-
-Ltac forward_call_id00_wow'  :=
-let H := fresh in intro H;
-eapply (semax_call_id00_wow _ _ _ _ _ _ _ _ _ _ _ _ _ _ _ _ _ _ _ _ _ _ _ _ _ _ _ H); 
- clear H;
- lazymatch goal with Frame := _ : list mpred |- _ => try clear Frame end;
- [ check_result_type 
- | cbv beta iota zeta; unfold_post; extensionality rho;
-    repeat rewrite exp_uncurry;
-    try rewrite no_post_exists0;
-    repeat rewrite exp_unfold;
-    first [reflexivity | extensionality; simpl; reflexivity | give_EX_warning]
- | unify_postcondition_exps
- | unfold fold_right_and; repeat rewrite and_True; auto
- ].
-
-Ltac fwd_call'_dep ts witness :=
-lazymatch goal with
-| |- semax _ _ (Ssequence (Scall _ _ _) _) _ =>
-  eapply semax_seq';
-    [prove_call_setup' ts witness;
-     clear_Delta_specs; clear_MORE_POST;
-     [ .. | 
-      lazymatch goal with
-      | |- _ -> semax _ _ (Scall (Some _) _ _) _ =>
-         forward_call_id1_wow'
-      | |- call_setup2' _ _ _ _ _ _ _ _ _ ?retty _ _ _ _ _ _ _ _ _ _ _ _ _ _ _ _ _ -> 
-                semax _ _ (Scall None _ _) _ =>
-        tryif (unify retty Tvoid)
-        then forward_call_id00_wow'
-        else forward_call_id01_wow'
-     end]
-   | after_forward_call ]
-| |- semax _ _ (Ssequence (Ssequence (Scall (Some ?ret') _ _)
-                                       (Sset _ (Ecast (Etempvar ?ret'2 _) _))) _) _ =>
-       unify ret' ret'2;
-       eapply semax_seq';
-         [prove_call_setup' ts witness;
-          clear_Delta_specs; clear_MORE_POST;
-             [ .. | forward_call_id1_x_wow' ]
-         |  after_forward_call ]
-| |- semax _ _ (Ssequence (Ssequence (Scall (Some ?ret') _ _)
-                                       (Sset _ (Etempvar ?ret'2 _))) _) _ =>
-       unify ret' ret'2;
-       eapply semax_seq';
-         [prove_call_setup' ts witness;
-          clear_Delta_specs; clear_MORE_POST;
-             [ .. | forward_call_id1_y_wow' ]
-         |  after_forward_call ]
-| |- _ => rewrite <- seq_assoc; fwd_call'_dep ts witness
-end.
-
-Ltac fwd_call_dep ts witness :=
- try lazymatch goal with
-      | |- semax _ _ (Scall _ _ _) _ => rewrite -> semax_seq_skip
-      end;
- repeat lazymatch goal with
-  | |- semax _ _ (Ssequence (Ssequence (Ssequence _ _) _) _) _ =>
-      rewrite <- seq_assoc
- end;
-lazymatch goal with |- @semax ?CS _ ?Delta _ (Ssequence ?C _) _ =>
-  lazymatch C with context [Scall _ _ _] =>
-         fwd_call'_dep ts witness
-    end
-end.
-
-Tactic Notation "forward_call_dep" constr(ts) constr(witness) := fwd_call_dep ts witness.
-
-Lemma node_entry_duplicable : forall v vs locs g lg lg' i, duplicable (node_entry v vs locs g lg lg' i).
+Lemma node_entry_duplicable : forall L locs g lg lg' i, duplicable (node_entry L locs g lg lg' i).
 Proof.
   intros; unfold node_entry.
-  apply exp_duplicable; intro.
-  apply prop_duplicable, protocol_R_duplicable.
+  apply protocol_R_duplicable.
 Qed.
 
 Lemma version_T_duplicable : forall locs g lg lg' s v, duplicable (version_T locs g lg lg' s v).
 Proof.
   intros; unfold version_T.
   apply prop_duplicable, exp_duplicable; intro.
-  apply sepcon_list_duplicable.
+  apply prop_duplicable, sepcon_list_duplicable.
   rewrite Forall_map, Forall_forall; intros; apply node_entry_duplicable.
 Qed.
 
-Definition map_add {A B} (m1 m2 : A -> option B) v := match m1 v with Some v' => Some v' | None => m2 v end.
-
-Lemma log_join_spec : forall m1 m2 m3, join m1 m2 m3 -> m3 = map_add m1 m2.
+Lemma map_Znth_add : forall {A B} (m1 m2 : A -> option (list B)) i d,
+  map_Znth i (map_add m1 m2) d = map_add (map_Znth i m1 d) (map_Znth i m2 d).
 Proof.
-  simpl; intros.
-  extensionality x; unfold map_add.
-  destruct (m1 x) eqn: Hm1.
-  - rewrite H; auto.
-  - destruct (m2 x) eqn: Hm2.
-    + rewrite H; auto.
-    + destruct (m3 x) eqn: Hm3; auto.
-      rewrite H in Hm3; destruct Hm3 as [Hm3 | Hm3]; rewrite Hm3 in *; discriminate.
+  intros; unfold map_add, map_Znth; extensionality.
+  destruct (m1 x); auto.
 Qed.
 
-Lemma map_add_incl_compat : forall m1 m2 m3, log_incl m1 m2 -> log_incl (map_add m3 m1) (map_add m3 m2).
-Proof.
-  unfold map_add; repeat intro.
-  destruct (m3 v1); auto.
-Qed.
-
-Lemma node_entry_choose : forall v1 v2 vs1 vs2 locs g lg lg' i,
-  view_shift (node_entry v1 vs1 locs g lg lg' i * node_entry v2 vs2 locs g lg lg' i)
-             (node_entry v1 vs1 locs g lg lg' i).
+Lemma node_entry_join : forall L1 L2 locs g lg lg' i,
+  node_entry L1 locs g lg lg' i * node_entry L2 locs g lg lg' i |-- node_entry (map_add L1 L2) locs g lg lg' i.
 Proof.
   intros; unfold node_entry.
-  view_shift_intro log1; view_shift_intro log2; view_shift_intros.
-  etransitivity; [apply protocol_R_choose | apply derives_view_shift; Exists log1; entailer!].
-  intros ??? Hincl Hjoin.
-  apply join_comm in Hjoin.
-  pose proof (log_join_spec _ _ _ Hjoin); subst.
-  exists (map_add s' log1); split; [|apply map_add_incl_compat; auto].
-  repeat intro; unfold map_add.
-  destruct (s' v0) eqn: Hin; split; auto; intros [|]; auto; try discriminate.
-  exploit Hincl; eauto; intro.
-  simpl in Hjoin.
-  assert (map_add s' s2 v0 = Some z) as Hin' by (rewrite Hjoin; auto).
-  assert (map_add s' s2 v0 = Some v3) as Hin2 by (rewrite Hjoin; auto).
-  rewrite Hin' in Hin2; inv Hin2; auto.
+  eapply derives_trans; [apply protocol_R_join'|].
+  Intros L; apply map_join_spec in H; subst; auto.
 Qed.
 
 Definition list_max v l := fold_right Z.max v l.
@@ -1057,58 +332,91 @@ Proof.
     + etransitivity; eauto; apply Zle_max_l.
 Qed.
 
-Lemma log_incl_latest : forall v1 v2 v1' v2' log log' (Hincl : log_incl log log')
-  (Hlatest : log_latest log v1 v2) (Hlatest' : log_latest log' v1' v2'), v1 <= v1'.
+Lemma node_state_duplicable : forall L version locs g g' lg lg',
+  duplicable (node_state L version locs g g' lg lg').
 Proof.
-  intros.
-  destruct (zlt v1' v1); [|omega].
-  destruct Hlatest' as (? & Hlatest').
-  specialize (Hlatest' _ l).
-  destruct Hlatest as (Hv1 & _); specialize (Hincl _ _ Hv1).
-  rewrite Hincl in Hlatest'; discriminate.
-Qed.
-
-Lemma node_state_duplicable : forall v vs version locs g g' lg lg',
-  duplicable (node_state v vs version locs g g' lg lg').
-Proof.
-  intros; apply sepcon_duplicable.
+  intros; unfold node_state.
+  apply exp_duplicable; intro v.
+  apply exp_duplicable; intro vs.
+  apply sepcon_duplicable.
   - apply prop_duplicable, protocol_R_duplicable.
   - apply sepcon_list_duplicable; rewrite Forall_map, Forall_forall; intros; simpl.
     apply node_entry_duplicable.
 Qed.
 
+Lemma node_state_join : forall L1 L2 version locs g g' lg lg',
+  node_state L1 version locs g g' lg lg' * node_state L2 version locs g g' lg lg' |--
+  node_state (map_add L1 L2) version locs g g' lg lg'.
+Proof.
+  intros; unfold node_state.
+  Intros v1 vs1 v2 vs2.
+  rewrite <- sepcon_assoc, (sepcon_comm _ (protocol_R _ _ _ _ _ _)), <- sepcon_assoc.
+  erewrite protocol_R_join; [|simpl; eauto].
+  rewrite Z.max_comm; Exists (Z.max v1 v2) (if zlt v1 v2 then vs2 else vs1); entailer!.
+  { split; [|apply log_latest_add; auto].
+    destruct (Z.max_spec v1 v2) as [[? ->] | [? ->]]; auto. }
+  rewrite <- sepcon_map; apply sepcon_list_derives; rewrite !Zlength_map; auto; intros.
+  erewrite !Znth_map, !Znth_upto by (auto; rewrite Zlength_upto in *; omega).
+  rewrite map_Znth_add; apply node_entry_join.
+Qed.
+
+Lemma node_entry_single : forall log locs g lg lg' i v v', log v = Some v' ->
+  view_shift (node_entry log locs g lg lg' i) (node_entry (singleton v v') locs g lg lg' i).
+Proof.
+  intros; unfold node_entry; apply protocol_R_forget.
+  - intros ?? Hincl Hjoin; apply join_comm in Hjoin; pose proof (map_join_spec _ _ _ Hjoin); subst.
+    do 2 eexists; [|apply map_add_incl_compat; eauto].
+    specialize (Hincl v); unfold singleton in *.
+    rewrite eq_dec_refl in Hincl; specialize (Hincl _ eq_refl).
+    repeat intro; simpl in *.
+    specialize (Hjoin v1).
+    unfold singleton, map_add, map_Znth in *.
+    if_tac; subst; simpl.
+    + destruct (s' v); split; auto; intros [X | X]; auto; try discriminate.
+      inv X; apply Hjoin; auto.
+    + destruct (s' v1); split; auto; intros [|]; auto; discriminate.
+  - unfold singleton, map_Znth; intros ??; if_tac; [|discriminate].
+    intro X; inv X; rewrite H; auto.
+Qed.
+
 Lemma body_read : semax_body Vprog Gprog f_read read_spec.
 Proof.
   start_atomic_function.
-  destruct x as (((((((((((n, out), sh), shi), version), locs), g), g'), lg), lg'), v0), vs0); Intros.
+  destruct x as (((((((((n, out), sh), shi), version), locs), g), g'), lg), lg'); Intros.
   destruct H as (HP0 & HP & HQ).
   rewrite map_map in HP, HQ.
   assert (0 <= size) by (rewrite size_def; computable).
-  apply semax_pre with (P' := EX v : Z, EX vers : list Z,
-    PROP (Forall (fun v' => Z.even v' = true /\ v' - 1 <= v) vers; Zlength vers = size)
-    LOCAL (temp _n n; temp _out out)
+  gather_SEP 3 2.
+  rewrite <- (map_map II); apply invariants_view_shift with
+    (Q0 := (EX L : _, node_state L version locs g g' lg lg') * P).
+  { rewrite map_map, sepcon_comm; etransitivity; [apply HP|].
+    etransitivity; [|rewrite sepcon_assoc, (sepcon_comm P); apply view_shift_sepcon2, HP].
+    view_shift_intro L.
+    etransitivity; [apply view_shift_sepcon1, node_state_duplicable|].
+    apply derives_view_shift; Exists L L; cancel. }
+  Intros L; rewrite map_map.
+  apply semax_pre with (P' := PROP () LOCAL (temp _n n; temp _out out)
     SEP (@data_at CompSpecs sh tnode (version, locs) n; data_at_ shi (tarray tint size) out;
-         protocol_R version g g' v Z.le (version_T locs g lg lg');
-         EX vals : list Z, fold_right sepcon emp (map (fun i => node_entry (Znth i vers 0) vals locs g lg lg' i)
-             (upto (Z.to_nat size))); fold_right sepcon emp (map (fun p : Z => invariant (II p)) lI); P)).
-  { Exists v0 (repeat v0 (Z.to_nat size)) vs0; unfold node_state; entailer!.
-    { split; [apply Forall_repeat; split; auto; omega | rewrite Zlength_repeat, Z2Nat.id; auto]. }
+         EX v : Z, protocol_R version g g' v Z.le (version_T locs g lg lg');
+         EX ll : _, fold_right sepcon emp (map (fun i => node_entry (Znth i ll empty_map) locs g lg lg' i)
+           (upto (Z.to_nat size)));
+         fold_right sepcon emp (map (fun p : Z => invariant (II p)) lI); P)).
+  { unfold node_state; Intros v vs.
+    Exists v (map (fun i => map_Znth i L 0) (upto (Z.to_nat size))); entailer!.
     erewrite map_ext_in; eauto; intros; simpl.
-    rewrite In_upto in *; rewrite Znth_repeat'; auto. }
+    rewrite In_upto in *; erewrite Znth_map, Znth_upto; rewrite ?Zlength_upto; auto; omega. }
   eapply semax_loop; [|forward; unfold loop2_ret_assert; apply drop_tc_environ].
-  Intros v vers vals.
+  Intros v ll.
   repeat forward.
-  forward_call_dep [Z : Type] (version, g, g', v, Z.le, version_T locs g lg lg',
-    fold_right sepcon emp (map (fun i => node_entry (Znth i vers 0) vals locs g lg lg' i) (upto (Z.to_nat size))),
-    version_T locs g lg lg').
+  forward_call_dep [Z : Type] (version, g, g', v, Z.le, version_T locs g lg lg', emp, version_T locs g lg lg').
   { split; intros; [|apply version_T_duplicable].
     etransitivity; [apply view_shift_sepcon2, version_T_duplicable|].
     rewrite <- sepcon_assoc; reflexivity. }
-  unfold version_T at 2; Intros x vs1; destruct x as (v1', v1); simpl in *; subst.
-  gather_SEP 2 1; rewrite <- sepcon_map; eapply view_shift_sepcon_list with (l2 := map _ (upto (Z.to_nat size)));
+  unfold version_T at 2; Intros x L1; destruct x as (v1', v1); simpl in *; subst.
+  gather_SEP 2 5; rewrite <- sepcon_map; eapply view_shift_sepcon_list with (l2 := map _ (upto (Z.to_nat size)));
     rewrite ?Zlength_map; auto; intros.
   { erewrite !Znth_map, !Znth_upto by (auto; rewrite ?Zlength_upto in *; omega).
-    apply node_entry_choose. }
+    apply derives_view_shift, node_entry_join. }
   match goal with |-semax _ (PROP () (LOCALx ?Q (SEPx ?R))) _ _ =>
     forward_if (PROP (Z.even v1 = true) (LOCALx Q (SEPx R))) end.
   { eapply semax_pre; [|apply semax_continue].
@@ -1118,26 +426,25 @@ Proof.
     go_lower.
     unfold Int.one in *; rewrite and_repr, land_1, Zmod_even in *.
     destruct (Z.even v1) eqn: Hodd; try contradiction.
-    Exists v1 (repeat (v1 - 1) (Z.to_nat size)) vs1; entailer!.
-    { split; [apply Forall_repeat; rewrite Z.even_sub, Hodd; split; auto; omega|].
-      rewrite Zlength_repeat, Z2Nat.id; auto. }
-    erewrite map_ext_in; eauto; simpl; intros.
-    rewrite In_upto in *; rewrite Znth_repeat'; auto. }
+    Exists v1 (map (fun i => map_add (map_Znth i L1 0) (Znth i ll empty_map)) (upto (Z.to_nat size))); entailer!.
+    erewrite map_ext_in; eauto; intros; simpl.
+    rewrite In_upto in *; erewrite Znth_map, Znth_upto; rewrite ?Zlength_upto; auto; omega. }
   { forward.
     entailer!.
     unfold Int.one in *; rewrite and_repr, land_1, Zmod_even in *.
     destruct (Z.even v1); auto; discriminate. }
   Intros.
-  replace (Z.even v1) with true.
+  destruct (Z.even v1) eqn: Hv1; try discriminate.
   forward_for_simple_bound 8 (EX i : Z, EX vals : list Z, PROP (Zlength vals = i)
     LOCAL (temp _snap (vint v1); temp _ver version; temp _n n; temp _out out)
     SEP (@data_at CompSpecs sh tnode (version, locs) n;
          data_at shi (tarray tint size) (map (fun x => vint x) vals ++ repeat Vundef (Z.to_nat (size - i))) out;
          EX vers' : list Z, !!(Zlength vers' = i /\ Forall (fun v => Z.even v = true /\ v1 <= v) vers') &&
            protocol_R version g g' (list_max v1 (map (fun x => x - 1) vers')) Z.le (version_T locs g lg lg') *
-           fold_right sepcon emp (map (fun i => node_entry (Znth i vers' 0) vals locs g lg lg' i)
+           fold_right sepcon emp (map (fun i => node_entry (singleton (Znth i vers' 0) (Znth i vals 0)) locs g lg lg' i)
              (sublist 0 i (upto (Z.to_nat size))));
-         fold_right sepcon emp (map (node_entry v1 vs1 locs g lg lg') (sublist i size (upto (Z.to_nat size))));
+         fold_right sepcon emp (map (fun i => node_entry (map_add (map_Znth i L1 0) (Znth i ll empty_map))
+           locs g lg lg' i) (sublist i size (upto (Z.to_nat size))));
          fold_right sepcon emp (map (fun p : Z => invariant (II p)) lI); P)).
   { Exists (@nil Z) (@nil Z).
     rewrite data_at__eq; unfold default_val; simpl data_at.
@@ -1151,12 +458,11 @@ Proof.
       eapply Forall_impl; [|eauto]; auto. }
     { rewrite <- size_def; apply prop_right; auto. }
     erewrite sublist_next with (i0 := i), Znth_upto by (rewrite ?Zlength_upto, ?Z2Nat.id; auto; omega); simpl.
-    unfold node_entry; Intros log.
-    Print node_entry.
-    forward_call_dep [Z -> option Z : Type] (Znth i locs Vundef, Znth i lg Vundef, Znth i lg' Vundef, log,
-      log_incl, data_T g,
+    unfold node_entry at 2.
+    forward_call_dep [Z -> option Z : Type] (Znth i locs Vundef, Znth i lg Vundef, Znth i lg' Vundef,
+      map_add (map_Znth i L1 0) (Znth i ll empty_map), @map_incl Z Z, data_T g,
       protocol_R version g g' (list_max v1 (map (fun x => x - 1) vers')) Z.le (version_T locs g lg lg'),
-      fun s v => EX v' : Z, !!(Z.even v' = true /\ log_latest s v' v) &&
+      fun s (v : Z) => EX v' : Z, !!(Z.even v' = true /\ log_latest s v' v) &&
         protocol_R version g g' (list_max v1 (map (fun x => x - 1) (vers' ++ [v']))) Z.le (version_T locs g lg lg')).
     { split; [|intros; apply exp_duplicable; intro; apply prop_duplicable, protocol_R_duplicable].
       intros; unfold data_T.
@@ -1168,18 +474,23 @@ Proof.
       rewrite map_app, list_max_app; simpl.
       rewrite Z.max_comm, list_max_max; auto. }
     Intros y v'; destruct y as (d, log'); simpl in *.
+    eapply node_entry_single.
+    { match goal with H : log_latest _ _ _ |- _ => destruct H; eauto end. }
     gather_SEP 1 2; rewrite protocol_R_R.
     forward.
     go_lower; Exists (x ++ [d]) (vers' ++ [v']); rewrite !Zlength_app, !Zlength_cons, !Zlength_nil.
+    match goal with H : exists vs, log_latest _ _ _ |- _ => destruct H as (vs1 & HL1) end.
     rewrite <- size_def, upd_init, !map_app, <- app_assoc by (rewrite ?Zlength_map; omega);
       unfold node_entry; entailer!.
     { rewrite Forall_app; repeat constructor; auto.
-      eapply log_incl_latest; eauto. }
+      eapply log_incl_latest; eauto.
+      unfold map_Znth, map_add.
+      destruct HL1 as [->]; simpl; eauto. }
     rewrite sublist_split with (mid := Zlength x)(hi := Zlength x + 1)
       by (rewrite ?Zlength_upto, ?Z2Nat.id; simpl; omega).
     erewrite sublist_len_1, Znth_upto by (rewrite ?Zlength_upto, ?Z2Nat.id; simpl; omega).
     rewrite map_app, sepcon_app; simpl.
-    Exists log'; rewrite !app_Znth2 by omega.
+    rewrite !app_Znth2 by omega.
     replace (Zlength vers') with (Zlength x); rewrite Zminus_diag, !Znth_0_cons; simpl; entailer!.
     apply sepcon_list_derives; rewrite !Zlength_map; auto.
     intros ? Hi; erewrite !Znth_map by auto.
@@ -1201,83 +512,79 @@ Proof.
     + subst.
       rewrite <- (map_map II).
       gather_SEP 0 5 8 7; rewrite <- !sepcon_assoc; apply invariants_view_shift with
-        (Q0 := node_state v1 vals' version locs g g' lg lg' * EX v : Z, EX vs : list Z, Q (v, vs) (v1, vals')).
+        (Q0 := EX L : _, Q L (v1, vals')).
       { rewrite !map_map, !sepcon_assoc, (sepcon_comm P), <- sepcon_assoc.
         etransitivity; [apply view_shift_sepcon2, HP|].
-        view_shift_intro x; destruct x as (vi, vsi).
-        rewrite <- exp_sepcon2.
-        etransitivity; [|apply view_shift_sepcon2; etransitivity; [apply (HQ (vi, vsi) (v1, vals')) |
-          apply derives_view_shift; Exists vi vsi; cancel]].
-        etransitivity; [apply view_shift_sepcon1|].
-        { etransitivity; [|apply (node_state_duplicable v1 vals' version locs g g' lg lg')].
-          apply derives_view_shift; unfold node_state; entailer!.
-          erewrite map_ext_in; eauto; intros; f_equal.
-          rewrite In_upto, Z2Nat.id in * by auto.
-          match goal with H : Forall _ vers' |- _ => apply Forall_Znth with (i := a)(d := 0) in H;
-            [destruct H as [Heven] | omega] end.
-          destruct (list_max_spec (map (fun x => x - 1) vers') v1) as [_ Hmax].
-          rewrite Forall_map in Hmax.
-          apply Forall_Znth with (i := a)(d := 0) in Hmax; [simpl in Hmax | omega].
-          destruct (eq_dec (Znth a vers' 0) (v1 + 1)); [|omega].
-          rewrite e, Z.even_add in Heven; replace (Z.even v1) with true in Heven; discriminate. }
-        apply derives_view_shift; fast_cancel. }
-      Intros vi vsi.
+        view_shift_intro L2.
+        etransitivity; [|etransitivity; [apply (HQ L2 (v1, vals')) | (* do we know a floor on v1? *)
+          apply derives_view_shift; Exists L2; cancel]].
+        apply derives_view_shift; cancel; unfold node_state.
+        Exists v1 vals'; entailer!.
+        { apply log_latest_singleton. }
+        erewrite map_ext_in; eauto; intros; simpl.
+        rewrite map_Znth_single.
+        rewrite In_upto, Z2Nat.id in * by auto.
+        match goal with H : Forall _ vers' |- _ => apply Forall_Znth with (i := a)(d := 0) in H;
+          [destruct H as [Heven] | omega] end.
+        destruct (list_max_spec (map (fun x => x - 1) vers') v1) as [_ Hmax].
+        rewrite Forall_map in Hmax.
+        apply Forall_Znth with (i := a)(d := 0) in Hmax; [simpl in Hmax | omega].
+        destruct (eq_dec (Znth a vers' 0) v1); subst; auto.
+        assert (Znth a vers' 0 = v1 + 1) as Heq by omega.
+        rewrite Heq, Z.even_add in Heven; replace (Z.even v1) with true in Heven; discriminate. }
+      Intros L2.
       forward.
-      rewrite map_map; Exists (v1, vals') (vi, vsi); entailer!.
+      rewrite map_map; Exists (v1, vals') L2; entailer!.
     + forward.
       entailer!.
     + intros; unfold overridePost.
       destruct (eq_dec ek EK_normal); [subst | apply drop_tc_environ].
       unfold POSTCONDITION, abbreviate, loop1_ret_assert.
-      Intros; go_lower; Exists v2 vers' vals'; entailer!.
-      rewrite Forall_forall; intros ? Hin.
-      split; [match goal with H : Forall _ vers' |- _ => rewrite Forall_forall in H; apply H; auto end|].
-      destruct (list_max_spec (map (fun x => x - 1) vers') v1) as (_ & Hle).
-      rewrite Forall_map, Forall_forall in Hle; specialize (Hle _ Hin); simpl in Hle; omega.
+      Intros; go_lower; Exists v2 (map (fun i => singleton (Znth i vers' 0) (Znth i vals' 0))
+        (upto (Z.to_nat size))); entailer!.
+      erewrite map_ext_in; eauto; intros; simpl.
+      rewrite In_upto in *; erewrite Znth_map, Znth_upto; rewrite ?Zlength_upto; auto; omega.
 Qed.
 
-(* up *)
-Definition map_upd (H : Z -> option Z) k v k' := if eq_dec k' k then Some v else H k'.
-
-Lemma log_latest_upd : forall log v1 v2 v1' v2', log_latest log v1 v2 -> v1 < v1' ->
-  log_incl log (map_upd log v1' v2') /\ log_latest (map_upd log v1' v2') v1' v2'.
-Proof.
-  intros; destruct H as (? & Hlast); unfold map_upd; split.
-  - repeat intro; if_tac; auto.
-    subst; rewrite (Hlast v1') in *; auto; discriminate.
-  - split; [rewrite eq_dec_refl; auto|].
-    intros v' ?; lapply (Hlast v'); [|omega].
-    intro; if_tac; auto; omega.
-Qed.
-
-Lemma update_entries : forall v v' vs vals locs g lg lg', view_shift
-  (fold_right sepcon emp (map (fun j => EX log : _, !! log_latest log v' (Znth j vals 0) &&
-     protocol_W (Znth j locs Vundef) (Znth j lg Vundef) (Znth j lg' Vundef) log log_incl (data_T g))
-     (upto (Z.to_nat size))) *
-   fold_right sepcon emp (map (node_entry v vs locs g lg lg') (upto (Z.to_nat size))))
-  (fold_right sepcon emp (map (fun j => EX log : _, !! log_latest log v' (Znth j vals 0) &&
-     protocol_W (Znth j locs Vundef) (Znth j lg Vundef) (Znth j lg' Vundef) log log_incl (data_T g))
-     (upto (Z.to_nat size))) *
-   fold_right sepcon emp (map (node_entry v' vals locs g lg lg') (upto (Z.to_nat size)))).
+Lemma update_entries : forall L ll locs g lg lg', view_shift
+  (fold_right sepcon emp (map (node_entry_W L locs g lg lg') (upto (Z.to_nat size))) *
+   fold_right sepcon emp (map (fun i => node_entry (map_Znth i ll 0) locs g lg lg' i) (upto (Z.to_nat size))))
+  (fold_right sepcon emp (map (node_entry_W L locs g lg lg') (upto (Z.to_nat size))) *
+   fold_right sepcon emp (map (fun i => node_entry (map_Znth i L 0) locs g lg lg' i) (upto (Z.to_nat size)))).
 Proof.
   intros.
   rewrite <- !sepcon_map.
   apply view_shift_sepcon_list; rewrite !Zlength_map; auto; intros.
   erewrite !Znth_map, !Znth_upto by (auto; rewrite ?Zlength_upto in *; omega).
-  unfold node_entry.
-  view_shift_intro log'; view_shift_intro log; view_shift_intros.
+  unfold node_entry, node_entry_W.
   etransitivity; [apply protocol_R_W|].
-  view_shift_intros; etransitivity; [apply protocol_W_R|].
-  apply derives_view_shift; Exists log' log'; entailer!.
+  view_shift_intros; apply protocol_W_R.
+Qed.
+
+Lemma map_Znth_log_latest : forall {B} m k (v : list B) i d, log_latest m k v ->
+  log_latest (map_Znth i m d) k (Znth i v d).
+Proof.
+  unfold log_latest, map_Znth; intros.
+  destruct H as [-> H]; split; auto.
+  intros; rewrite H; auto.
+Qed.
+
+Lemma map_Znth_upd : forall {A B} {A_eq : EqDec A} (m : A -> option (list B)) k v i d,
+  map_Znth i (map_upd m k v) d = map_upd (map_Znth i m d) k (Znth i v d).
+Proof.
+  intros; unfold map_Znth, map_upd; extensionality.
+  if_tac; auto.
 Qed.
 
 Lemma body_write : semax_body Vprog Gprog f_write write_spec.
 Proof.
   start_atomic_function.
-  destruct x as ((((((((((((n, input), sh), shi), version), locs), vals), g), g'), lg), lg'), v0), vs0); Intros.
+  destruct x as (((((((((((((n, input), sh), shi), version), locs), vals), g), g'), lg), lg'), L), v0), vs0); Intros.
   destruct H as (HP0 & HP & HQ).
   forward.
   rewrite map_map in HP, HQ.
+  unfold node_state_W; Intros v0' vs0'.
+  assert (v0' = v0 /\ vs0' = vs0) as [] by (eapply log_latest_inj; eauto); subst.
   focus_SEP 2; apply protocol_W_R.
   forward_call_dep [Z : Type] (version, g, g', v0, Z.le, version_T locs g lg lg',
     protocol_W version g g' v0 Z.le (version_T locs g lg lg'), fun s v : Z => !!(v = s) && emp).
@@ -1292,7 +599,8 @@ Proof.
   { split; [auto | split; [|omega]].
     intros.
     apply derives_view_shift; unfold version_T.
-    Intros vs; Exists vs; subst; rewrite Z.even_add, Z.add_simpl_r; replace (Z.even v0) with true; simpl; entailer!. }
+    Intros vs; Exists vs; subst.
+    rewrite Z.even_add, Z.add_simpl_r; replace (Z.even v0) with true in *; simpl; entailer!. }
   assert (0 <= size) by (rewrite size_def; computable).
   assert_PROP (Zlength (map (fun x => vint x) vals) = size) by entailer!.
   assert (Z.even (v0 + 2) = true) by (rewrite Z.even_add; replace (Z.even v0) with true; auto).
@@ -1300,12 +608,8 @@ Proof.
   focus_SEP 4.
   match goal with |-semax _ (PROP () (LOCALx ?Q (SEPx (_ :: ?R)))) _ _ =>
   forward_for_simple_bound 8 (EX i : Z, PROP () (LOCALx Q
-    (SEPx (fold_right sepcon emp (map (fun j => EX log : _, !!(log_latest log (v0 + 2) (Znth j vals 0)) &&
-             protocol_W (Znth j locs Vundef) (Znth j lg Vundef) (Znth j lg' Vundef) log log_incl (data_T g))
-             (sublist 0 i (upto (Z.to_nat size)))) ::
-           fold_right sepcon emp (map (fun j => EX log : _, !!(log_latest log v0 (Znth j vs0 0)) &&
-             protocol_W (Znth j locs Vundef) (Znth j lg Vundef) (Znth j lg' Vundef) log log_incl (data_T g))
-             (sublist i size (upto (Z.to_nat size)))) :: R)))) end.
+    (SEPx (fold_right sepcon emp (map (node_entry_W (map_upd L (v0 + 2) vals) locs g lg lg') (sublist 0 i (upto (Z.to_nat size)))) ::
+           fold_right sepcon emp (map (node_entry_W L locs g lg lg') (sublist i size (upto (Z.to_nat size)))) :: R)))) end.
   { rewrite sublist_nil, sublist_same by (rewrite ?Zlength_upto, ?Z2Nat.id; auto).
     entailer!. }
   - (* loop body *)
@@ -1315,15 +619,16 @@ Proof.
       eapply Forall_impl; [|eauto]; auto. }
     forward.
     erewrite sublist_next with (i0 := i), Znth_upto by (rewrite ?Zlength_upto, ?Z2Nat.id; auto; omega); simpl.
-    Intros log.
     rewrite Zlength_map in *.
-    destruct (log_latest_upd log v0 (Znth i vs0 0) (v0 + 2) (Znth i vals 0)); auto; try omega.
+    destruct (log_latest_upd (map_Znth i L 0) v0 (Znth i vs0 0) (v0 + 2) (Znth i vals 0)); auto; try omega.
+    { apply map_Znth_log_latest; auto. }
+    unfold node_entry_W at 2.
     forward_call_dep [Z -> option Z : Type] (Znth i locs Vundef, Znth i vals 0, Znth i lg Vundef,
-      Znth i lg' Vundef, log, map_upd log (v0 + 2) (Znth i vals 0), log_incl, data_T g,
+      Znth i lg' Vundef, map_Znth i L 0, map_upd (map_Znth i L 0) (v0 + 2) (Znth i vals 0), @map_incl Z Z,
+      data_T g,
       protocol_W version g g' (v0 + 1) Z.le (version_T locs g lg lg'),
       protocol_W version g g' (v0 + 1) Z.le (version_T locs g lg lg')).
     { split; [apply Forall_Znth; auto; omega|].
-      destruct (log_latest_upd log v0 (Znth i vs0 0) (v0 + 2) (Znth i vals 0)); auto; try omega.
       split; auto; intros.
       unfold data_T.
       view_shift_intro ver; view_shift_intros.
@@ -1336,44 +641,285 @@ Proof.
       unfold protocol_W; rewrite general_atomics.invariant_duplicable at 3; entailer!. }
     erewrite sublist_split with (mid := i)(hi := i + 1), sublist_len_1, Znth_upto, map_app, sepcon_app
       by (rewrite ?Zlength_upto, ?Z2Nat.id; auto; omega); simpl fold_right.
-    rewrite <- size_def; Exists (map_upd log (v0 + 2) (Znth i vals 0)); entailer!.
+    rewrite <- size_def, <- map_Znth_upd; unfold node_entry_W; entailer!.
   - rewrite <- size_def, sublist_nil, sublist_same by (rewrite ?Zlength_upto, ?Z2Nat.id; auto; omega).
     assert (repable_signed (v0 + 2)) by admit.
+    destruct (log_latest_upd L v0 vs0 (v0 + 2) vals); auto; try omega.
     forward_call_dep [Z : Type] (version, v0 + 2, g, g', v0 + 1, v0 + 2, Z.le, version_T locs g lg lg',
-      fold_right sepcon emp (map (fun j => EX log : _, !! log_latest log (v0 + 2) (Znth j vals 0) &&
-        protocol_W (Znth j locs Vundef) (Znth j lg Vundef) (Znth j lg' Vundef) log log_incl (data_T g))
-        (upto (Z.to_nat size))),
-      fold_right sepcon emp (map (fun j => EX log : _, !! log_latest log (v0 + 2) (Znth j vals 0) &&
-        protocol_W (Znth j locs Vundef) (Znth j lg Vundef) (Znth j lg' Vundef) log log_incl (data_T g))
-        (upto (Z.to_nat size)))).
+      fold_right sepcon emp (map (node_entry_W (map_upd L (v0 + 2) vals) locs g lg lg') (upto (Z.to_nat size))),
+      fold_right sepcon emp (map (node_entry_W (map_upd L (v0 + 2) vals) locs g lg lg') (upto (Z.to_nat size)))).
     { fast_cancel. }
     { split; [auto | split; [|omega]].
       intros; unfold version_T.
-      view_shift_intro vs.
+      view_shift_intro L1; view_shift_intros.
       etransitivity; [apply update_entries|].
       rewrite Z.even_add; replace (Z.even v0) with true; simpl.
-      apply derives_view_shift; Exists vals; entailer!. }
+      apply derives_view_shift; Exists (map_upd L (v0 + 2) vals); entailer!.
+      eauto. }
     rewrite <- (map_map II).
     gather_SEP 0 1 6 5; rewrite <- !sepcon_assoc; apply invariants_view_shift with
-      (Q0 := protocol_W version g g' (v0 + 2) Z.le (version_T locs g lg lg') *
-        fold_right sepcon emp (map (fun j => EX log : _, !!(log_latest log (v0 + 2) (Znth j vals 0)) &&
-          protocol_W (Znth j locs Vundef) (Znth j lg Vundef) (Znth j lg' Vundef) log log_incl (data_T g))
-        (upto (Z.to_nat size))) * EX v : Z, EX vs : list Z, Q (v, vs) tt).
+      (Q0 := node_state_W (map_upd L (v0 + 2) vals) version locs g g' lg lg' * EX L : _, Q L tt).
     { rewrite !map_map, !sepcon_assoc, (sepcon_comm P), <- sepcon_assoc.
       etransitivity; [apply view_shift_sepcon2, HP|].
-      view_shift_intro x; destruct x as (v, vs).
+      view_shift_intro L1.
       rewrite <- !exp_sepcon2, <- exp_sepcon1, <- !sepcon_assoc.
-      rewrite !(sepcon_assoc (_ * _)), (sepcon_comm (exp _)), <- sepcon_assoc.
-      etransitivity; [|apply view_shift_sepcon2; etransitivity; [apply (HQ (v, vs) tt) |
-        apply derives_view_shift; Exists v vs; auto]].
-      unfold node_state; view_shift_intros.
+      rewrite !sepcon_assoc, (sepcon_comm (exp _)), <- sepcon_assoc.
+      etransitivity; [|apply view_shift_sepcon2; etransitivity; [apply (HQ L1 tt) |
+        apply derives_view_shift; Exists L1; auto]].
+      unfold node_state; view_shift_intro v; view_shift_intro vs; view_shift_intros.
       rewrite <- !sepcon_assoc, (sepcon_comm _ (protocol_R _ _ _ _ _ _)), <- sepcon_assoc, 2sepcon_assoc.
       rewrite (sepcon_comm (protocol_R _ _ _ _ _ _)).
       etransitivity; [apply view_shift_sepcon1, protocol_R_W|].
       view_shift_intros; etransitivity; [apply view_shift_sepcon1, protocol_W_R|].
       rewrite sepcon_comm, <- !sepcon_assoc, 2sepcon_assoc.
       etransitivity; [apply view_shift_sepcon1, update_entries|].
-      apply derives_view_shift; entailer!. }
-    forward.
-    rewrite map_map; Exists tt (v, vs); entailer!.
+      apply derives_view_shift; unfold node_state_W.
+      Exists (v0 + 2) (v0 + 2) vals vals; entailer!. }
+    Intro L1; forward.
+    rewrite map_map; Exists tt L1; entailer!.
 Admitted.
+
+Lemma body_make_node : semax_body Vprog Gprog f_make_node make_node_spec.
+Proof.
+  start_function.
+  forward_malloc tnode n.
+  forward_malloc tint p.
+  repeat forward.
+  apply ghost_alloc with (g := (@None Z, Some 0)); [apply master_init' | Intros g].
+  apply master_snap; Intros.
+  apply ghost_snap_le with (v1 := -1); [omega|].
+  forward_for_simple_bound 8 (EX i : Z, EX ld : list val, PROP (Zlength ld = i; Forall isptr ld)
+    LOCAL (temp _n n)
+    SEP (ghost_snap (-1) g; ghost_master 0 g; malloc_token Tsh (sizeof tint) p; data_at Tsh tint (vint 0) p;
+         malloc_token Tsh (sizeof tnode) n;
+         @data_at CompSpecs Tsh tnode (p, ld ++ repeat Vundef (Z.to_nat (8 - i))) n;
+         EX lg : list val, EX lg' : list val, !!(Zlength lg = i /\ Zlength lg' = i) &&
+           fold_right sepcon emp (map (fun i => node_entry_W (singleton 0 (repeat 0 (Z.to_nat size))) ld g lg lg' i *
+             node_entry (singleton 0 0) ld g lg lg' i) (upto (Z.to_nat i)));
+         fold_right sepcon emp (map (malloc_token Tsh (sizeof tint)) ld))).
+  { Exists (@nil val) (@nil val) (@nil val); entailer!; auto. }
+  - apply ghost_snap_duplicable.
+    Intros lg lg'.
+    forward_malloc tint d.
+    rewrite data_at__isptr; Intros.
+    forward.
+    gather_SEP 1 2; eapply view_shift_trans; [|apply (make_protocol d 0 (singleton 0 0) (data_T g)); auto|].
+    { unfold data_T.
+      apply derives_view_shift; Exists 0; entailer!.
+      apply log_latest_singleton. }
+    Intros gi gi'.
+    apply protocol_W_R.
+    forward.
+    Exists (x ++ [d]) (lg ++ [gi]) (lg' ++ [gi']); rewrite upd_init, <- app_assoc, !Zlength_app, !Zlength_cons,
+      !Zlength_nil by (auto; tauto).
+    rewrite Z2Nat.inj_add, upto_app, !map_app, !sepcon_app, Z2Nat.id by omega.
+    unfold node_entry_W at 3; unfold node_entry at 3; simpl fold_right.
+    rewrite !app_Znth2 by omega.
+    replace (Zlength lg) with i; replace (Zlength lg') with i; replace (Zlength x) with i;
+      rewrite Z.add_0_r, Zminus_diag, !Znth_0_cons.
+    rewrite map_Znth_single, Znth_repeat.
+    entailer!.
+    { rewrite Forall_app; repeat constructor; auto. }
+    cancel; erewrite map_ext_in; eauto; simpl; intros.
+    unfold node_entry_W, node_entry.
+    rewrite In_upto, <- Zlength_correct in *.
+    rewrite !app_Znth1 by omega; auto.
+  - Intros ld lg lg'.
+    rewrite <- size_def in *.
+    rewrite Zminus_diag, app_nil_r.
+    gather_SEP 0 1; apply master_snap_absorb_gen.
+    rewrite sepcon_map; Intros.
+    gather_SEP 2 0 6; eapply view_shift_trans;
+      [|apply (make_protocol'(ord := Z.le) p g 0 0 (version_T ld g lg lg')); auto|].
+    { unfold version_T.
+      apply derives_view_shift; Exists (singleton 0 (repeat 0 (Z.to_nat size))); simpl; entailer!.
+      { eexists; apply log_latest_singleton. }
+      erewrite map_ext; eauto; intros; simpl.
+      rewrite map_Znth_single, Znth_repeat; auto. }
+    forward.
+    unfold node_state_W.
+    Exists n p ld g g' lg lg' 0 (repeat 0 (Z.to_nat size)); entailer!.
+    apply log_latest_singleton.
+Qed.
+
+Lemma body_writer : semax_body Vprog Gprog f_writer writer_spec.
+Proof.
+  name data _data.
+  start_function.
+  rewrite data_at__eq; unfold default_val; simpl.
+  repeat forward.
+  change (field_at Tsh (tarray tint 8) [] _ data) with (data_at Tsh (tarray tint 8) (repeat (vint 0) 8) data).
+  forward_for_simple_bound 3 (EX i : Z,
+    PROP ()
+    LOCAL (lvar _data (tarray tint 8) data; temp _n n)
+    SEP (data_at Tsh (tarray tint 8) (repeat (vint i) 8) data; @data_at CompSpecs sh tnode (version, locs) n;
+         node_state_W (map_upd_list L (map (fun i => (v + 2 * (i + 1), repeat (i + 1) 8)) (upto (Z.to_nat i))))
+           version locs g g' lg lg')).
+  { entailer!. }
+  - Intros.
+    match goal with |-semax _ (PROP () (LOCALx ?Q (SEPx (_ :: ?R)))) _ _ =>
+    forward_for_simple_bound 8 (EX j : Z, PROP () (LOCALx Q
+      (SEPx (data_at Tsh (tarray tint 8) (repeat (vint (i + 1)) (Z.to_nat j) ++
+             repeat (vint i) (Z.to_nat (8 - j))) data :: R)))) end.
+    { entailer!. }
+    + forward.
+      { entailer!.
+        rewrite app_Znth2; rewrite Zlength_repeat, Z2Nat.id; try omega.
+        rewrite Zminus_diag, Znth_repeat' by (rewrite Z2Nat.id; omega); auto. }
+      rewrite app_Znth2; rewrite Zlength_repeat, Z2Nat.id; try omega.
+      rewrite Zminus_diag, Znth_repeat' by (rewrite Z2Nat.id; omega).
+      forward.
+      rewrite add_repr, upd_init_const by auto; entailer!.
+    + 
+    (* change_compspecs runs forever here *)
+Ltac lookup_spec_and_change_compspecs CS id ::=
+ tryif apply f_equal_Some
+ then
+   (match goal with |- ?A = ?B =>
+      let x := fresh "x" in set (x := A);
+      let y := fresh "y" in set (y := B);
+      hnf in x; subst x; subst y
+   end;
+   match goal with
+   | |- ?fs = _ => check_canonical_funspec (id,fs);
+      first [reflexivity |
+      match goal with
+       | |- mk_funspec _ _ ?t1 _ _ = mk_funspec _ _ ?t2 _ _ =>
+         first [unify t1 t2
+           | elimtype False; elimtype (Witness_type_of_forward_call_does_not_match_witness_type_of_funspec
+      t2 t1)]
+      end]
+   end)
+ else elimtype  (Cannot_find_function_spec_in_Delta id).
+
+Lemma node_state_W_R : forall L version locs g g' lg lg',
+  view_shift (node_state_W L version locs g g' lg lg')
+             (node_state_W L version locs g g' lg lg' * node_state L version locs g g' lg lg').
+Proof.
+  intros; unfold node_state_W.
+  view_shift_intro v; view_shift_intro vs; view_shift_intros.
+  etransitivity; [apply view_shift_sepcon1, protocol_W_R|].
+  etransitivity.
+  - apply view_shift_sepcon2, view_shift_sepcon_list; [rewrite 2Zlength_map; eauto | rewrite Zlength_map; intros].
+    erewrite 2Znth_map, 2Znth_upto by (auto; rewrite Zlength_upto in *; omega).
+    unfold node_entry_W; apply protocol_W_R.
+  - apply derives_view_shift; unfold node_state.
+    Exists v vs v vs; rewrite sepcon_map; entailer!.
+Qed.
+
+      (* This is a bit annoying: because write is specified as atomic with node_state, we need to have a
+         node_state to call it, even though it's subsumed by node_state_W. *)
+      focus_SEP 2; apply node_state_W_R.
+      forward_call (n, data, sh, Tsh, version, locs, repeat (i + 1) 8, g, g', lg, lg', map_upd_list L
+        (map (fun i => (v + 2 * (i + 1), repeat (i + 1) 8)) (upto (Z.to_nat i))), v + 2 * i,
+        if eq_dec i 0 then vs else repeat i 8,
+        node_state (map_upd_list L (map (fun i => (v + 2 * (i + 1), repeat (i + 1) 8)) (upto (Z.to_nat i))))
+          version locs g g' lg lg',
+        fun (_ : Z -> option (list Z)) (_ : unit) => EX L : _, node_state L version locs g g' lg lg',
+        fun _ : Z -> option (list Z) => emp, fun _ : Z => FF, @nil Z).
+      { entailer!.
+        { split; [|split].
+          * apply Forall_repeat.
+            split; [pose proof Int.min_signed_neg; omega|].
+            transitivity 3; [omega | computable].
+          * rewrite Z.even_add_mul_2; auto.
+          * split; [if_tac; auto; rewrite size_def; apply Zlength_repeat|].
+            eapply log_latest_upd_list; eauto; try omega.
+            -- if_tac.
+               { subst; rewrite Z.add_0_r; auto. }
+               rewrite <- (Z.sub_simpl_r i 1), Z2Nat.inj_add, upto_app, map_app by omega.
+               setoid_rewrite last_snoc.
+               rewrite Z2Nat.id, Z.add_0_r; auto; omega.
+            -- rewrite Forall_map, Forall_forall; intros; simpl.
+               rewrite In_upto, Z2Nat.id in *; omega. }
+        rewrite size_def, Zminus_diag, app_nil_r, map_repeat; simpl; cancel. }
+      { split; [|split].
+        * admit.
+        * admit.
+        * intros _ _.
+          apply derives_view_shift; Exists (map_upd (map_upd_list L (map (fun i0 =>
+            (v + 2 * (i0 + 1), repeat (i0 + 1) 8)) (upto (Z.to_nat i)))) (v + 2 * i + 2) (repeat (i + 1) 8));
+            cancel. }
+      Intros L0.
+      rewrite Z2Nat.inj_add, upto_app, map_app, map_upd_list_app by omega.
+      change (upto 1) with [0]; simpl map_upd_list.
+      rewrite Z2Nat.id, Z.add_0_r, Z.mul_add_distr_l, Z.add_assoc by omega.
+      rewrite <- size_def; entailer!.
+      admit.
+  - forward.
+    Exists data; rewrite size_def; entailer!.
+Admitted.
+
+(*Lemma body_reader : semax_body Vprog Gprog f_reader reader_spec.
+Proof.
+  name data _data.
+  start_function.
+  forward_call (n, data, sh, Tsh, version, locs, g, g', lg, lg', ghost_hist gsh ([] : hist) gh,
+    fun (_ : Z * list Z) '(v, vs) => EX h' : _, !!(add_events [] [HRead v vs] h') &&
+      ghost_hist gsh h' gh,
+    fun s => ghost_hist gsh ([] : hist) gh * EX hr : _, !!(apply_hist (0, repeat 0 (Z.to_nat size)) hr = Some s) &&
+      ghost_ref hr gh,
+    fun p => if eq_dec p 0 then node_inv gh version locs g g' lg lg' else FF, [0]).
+  { entailer!.
+    rewrite size_def, eq_dec_refl; simpl; cancel. }
+  { split; [|split].
+    * apply ghost_timeless.
+    * simpl.
+      admit. (* laters are messy *)
+    * intros (v0, vs0) (v1, vs1); simpl.
+      unfold node_inv.
+      view_shift_intro hr; view_shift_intros.
+      rewrite <- !sepcon_assoc, (sepcon_comm _ (ghost_ref _ _)).
+      rewrite <- !sepcon_assoc, (sepcon_comm _ (ghost_hist _ _ _)).
+      rewrite <- sepcon_assoc.
+      rewrite <- sepcon_assoc, sepcon_assoc.
+      etransitivity; [apply view_shift_sepcon1, hist_add' with (e := HRead v1 vs1); auto|].
+      apply derives_view_shift; Exists [(length hr, HRead v1 vs1)]; simpl; entailer!.
+      { apply add_events_1 with (h := []), hist_incl_lt; auto. }
+      eapply derives_trans, now_later.
+      Exists v1 vs1 (hr ++ [HRead v1 vs1]); entailer!.
+      rewrite apply_hist_app; replace (apply_hist _ _) with (Some (v0, vs0)); auto.
+      (* At this point, the proof fails: the state recorded in the invariant may not match the state we read
+         from. *)
+Abort.*)
+
+(*Lemma body_reader : semax_body Vprog Gprog f_reader reader_spec.
+Proof.
+  name data _data.
+  start_atomic_function.
+  destruct x as (((((((((n, sh), version), locs), g), g'), lg), lg'), gh), gsh); Intros.
+  destruct H as (HP0 & HP & HQ).
+  rewrite map_map in HP, HQ.
+  forward_call (n, data, sh, Tsh, version, locs, g, g', lg, lg', P,
+    fun (_ : Z * list Z) '(v1, vs1) => Q tt (v1, vs1),
+    fun s => EX hr : _, !!(apply_hist (0, repeat 0 (Z.to_nat size)) hr = Some s) && ghost_ref hr gh, II, lI).
+  { simpl; rewrite <- size_def; entailer!. }
+  { split; [|split].
+    * auto.
+    * simpl.
+      admit. (* laters are messy *)
+    * intros (v0, vs0) (v1, vs1); simpl.
+      rewrite map_map; etransitivity; [|apply HQ]; simpl.
+      (* This also fails: the history in the invariant may not have caught up with the value we read. *)
+Abort.*)
+
+Lemma body_reader : semax_body Vprog Gprog f_reader reader_spec.
+Proof.
+  name data _data.
+  start_function.
+  forward_call (n, data, sh, Tsh, version, locs, g, g', lg, lg', node_state L version locs g g' lg lg',
+    fun (_ : Z -> option (list Z)) '(v, vs) => EX L' : _, !!(L' v = Some vs) && node_state L' version locs g g' lg lg',
+    fun _ : Z -> option (list Z) => emp, fun _ : Z => FF, @nil Z).
+  { rewrite <- size_def; entailer!; cancel. }
+  { split; [|split].
+    * admit.
+    * admit.
+    * intros L' (v1, vs1).
+      rewrite sepcon_emp, sepcon_comm; apply derives_view_shift; eapply derives_trans; [apply node_state_join|].
+      Exists (map_add (singleton v1 vs1) L'); simpl; entailer!.
+      unfold map_add, singleton; rewrite eq_dec_refl; auto. }
+  Intro x; destruct x as ((v', vs'), ?); simpl; Intros L'.
+  forward.
+  Exists data v' vs'; entailer!.
+  { 
+Qed.
